Isabelle/04_Composed_operations/CNF_concurrency.thy
@@ -1695,6 +1695,92 @@ proof -
     using \<open>([p] ;\<^sub>c [q]) \<parallel> [r] = (p @ q) \<interleave> r\<close> \<open>[p] ;\<^sub>c [q] \<parallel> [r] = [p] ;\<^sub>c (q \<interleave> r)\<close> \<open>set ([p] ;\<^sub>c (q \<interleave> r)) \<subseteq> set ((p @ q) \<interleave> r)\<close> by auto
 qed
 
+lemma inter1: "set ((ps \<interleave> qs) ;\<^sub>c (rs \<interleave> vs)) \<subseteq> set ((ps @ rs) \<interleave> (qs @ vs))"
+proof (induction ps arbitrary: qs rs vs)
+  case Nil
+  then show ?case apply auto
+    using comp_prop prop9_1 by fastforce
+next
+  case Cons1: (Cons p ps)
+  then show "set (((p # ps) \<interleave> qs) ;\<^sub>c (rs \<interleave> vs)) \<subseteq> set (((p # ps) @ rs) \<interleave> (qs @ vs))"
+  proof (induction qs arbitrary: rs vs)
+    case Nil
+    then show ?case apply auto
+      by (metis (no_types, lifting) Cons_eq_appendI comp_prop inter_perm list.discI list.set_cases permutation_set_equality prop9_1 set_ConsD)
+  next
+    case Cons2: (Cons q qs)
+    have "(\<And>qs rs vs. set ((ps \<interleave> qs) ;\<^sub>c (rs \<interleave> vs)) \<subseteq> set ((ps @ rs) \<interleave> (qs @ vs)))"
+      using Cons1 by auto
+    have "set ((ps \<interleave> qs) ;\<^sub>c (rs \<interleave> vs)) \<subseteq> set ((ps @ rs) \<interleave> (qs @ vs))"
+      by (simp add: Cons1)
+    have IH1: "set (((p # ps) \<interleave> qs) ;\<^sub>c (rs \<interleave> vs)) \<subseteq> set (((p # ps) @ rs) \<interleave> (qs @ vs))"
+      using Cons1 Cons2.IH by auto
+    from Cons2 show ?case using IH1
+    proof (induction rs arbitrary: vs)
+      case Nil
+      have "set (((p # ps) \<interleave> qs) ;\<^sub>c (rs \<interleave> vs)) \<subseteq> set (((p # ps) @ rs) \<interleave> (qs @ vs))"
+        using Cons1 Cons2.IH by blast
+      have "set ((ps \<interleave> qs) ;\<^sub>c (rs \<interleave> vs)) \<subseteq> set ((ps @ rs) \<interleave> (qs @ vs))"
+        by (simp add: Cons1)
+      have "set (((p # ps) \<interleave> qs) ;\<^sub>c ([] \<interleave> vs)) \<subseteq> set (((p # ps) @ []) \<interleave> (qs @ vs))"
+        using Nil.prems(3) by auto
+      then have "set (((p # ps) \<interleave> (q # qs)) ;\<^sub>c [vs]) \<subseteq> set (((p # ps)) \<interleave> ((q # qs) @ vs))"
+        apply (induction vs) apply (auto simp: composition_cnf_def)
+        by (metis Cons_eq_appendI prop9 rev_image_eqI)
+      then show "set (((p # ps) \<interleave> (q # qs)) ;\<^sub>c ([] \<interleave> vs)) \<subseteq> set (((p # ps) @ []) \<interleave> ((q # qs) @ vs))"
+        by simp
+    next
+      case Cons3: (Cons r rs)
+
+      have "((p # ps) @ r # rs) \<interleave> ((q # qs) @ vs) = map ((#) p) ((ps @ r # rs) \<interleave> (q # qs @ vs)) @ map ((#) q) ((p # ps @ r # rs) \<interleave> (qs @ vs))" by simp
+
+      have "(p # ps) \<interleave> (q # qs) = map ((#) p) (ps \<interleave> (q # qs)) @ map ((#) q) ((p # ps) \<interleave> qs)" by simp
+      have "((p # ps) \<interleave> (q # qs)) ;\<^sub>c ((r # rs) \<interleave> vs) = (map ((#) p) (ps \<interleave> (q # qs)) ;\<^sub>c ((r # rs) \<interleave> vs)) @ (map ((#) q) ((p # ps) \<interleave> qs) ;\<^sub>c ((r # rs) \<interleave> vs))" by (auto simp: composition_cnf_def)
+      
+      have "set ((ps \<interleave> (q # qs)) ;\<^sub>c ((r # rs) \<interleave> vs)) \<subseteq> set ((ps @ r # rs) \<interleave> (q # qs @ vs))"
+        using Cons1 by fastforce
+      then have "set ((map ((#) p) (ps \<interleave> (q # qs)) ;\<^sub>c ((r # rs) \<interleave> vs))) \<subseteq> set  (map ((#) p) ((ps @ r # rs) \<interleave> (q # qs @ vs)))" by (auto simp: composition_cnf_def)
+      have "set (((p # ps) \<interleave> qs) ;\<^sub>c ((r # rs) \<interleave> vs)) \<subseteq> set ((p # ps @ r # rs) \<interleave> (qs @ vs))"
+        using Cons3.prems(3) by auto
+      then have "set ((map ((#) q) ((p # ps) \<interleave> qs) ;\<^sub>c ((r # rs) \<interleave> vs))) \<subseteq> set ( map ((#) q) ((p # ps @ r # rs) \<interleave> (qs @ vs)))" by (auto simp: composition_cnf_def)
+      have "set ((map ((#) p) (ps \<interleave> (q # qs)) ;\<^sub>c ((r # rs) \<interleave> vs))) \<union> set ((map ((#) q) ((p # ps) \<interleave> qs) ;\<^sub>c ((r # rs) \<interleave> vs))) \<subseteq>
+            set  (map ((#) p) ((ps @ r # rs) \<interleave> (q # qs @ vs)))     \<union> set ( map ((#) q) ((p # ps @ r # rs) \<interleave> (qs @ vs)))"
+        using \<open>set (map ((#) p) (ps \<interleave> (q # qs)) ;\<^sub>c ((r # rs) \<interleave> vs)) \<subseteq> set (map ((#) p) ((ps @ r # rs) \<interleave> (q # qs @ vs)))\<close> \<open>set (map ((#) q) ((p # ps) \<interleave> qs) ;\<^sub>c ((r # rs) \<interleave> vs)) \<subseteq> set (map ((#) q) ((p # ps @ r # rs) \<interleave> (qs @ vs)))\<close> by blast
+      show "set (((p # ps) \<interleave> (q # qs)) ;\<^sub>c ((r # rs) \<interleave> vs)) \<subseteq> set (((p # ps) @ r # rs) \<interleave> ((q # qs) @ vs))"
+        using \<open>((p # ps) \<interleave> (q # qs)) ;\<^sub>c ((r # rs) \<interleave> vs) = map ((#) p) (ps \<interleave> (q # qs)) ;\<^sub>c ((r # rs) \<interleave> vs) @ map ((#) q) ((p # ps) \<interleave> qs) ;\<^sub>c ((r # rs) \<interleave> vs)\<close> \<open>set (map ((#) p) (ps \<interleave> (q # qs)) ;\<^sub>c ((r # rs) \<interleave> vs)) \<union> set (map ((#) q) ((p # ps) \<interleave> qs) ;\<^sub>c ((r # rs) \<interleave> vs)) \<subseteq> set (map ((#) p) ((ps @ r # rs) \<interleave> (q # qs @ vs))) \<union> set (map ((#) q) ((p # ps @ r # rs) \<interleave> (qs @ vs)))\<close> by auto
+    qed
+  qed
+qed
+
+lemma prop10_3_1: "set ([p] \<parallel> [q] ;\<^sub>c [r] \<parallel> [v]) \<subseteq> set (([p] ;\<^sub>c [r]) \<parallel> ([q] ;\<^sub>c [v]))"
+proof -
+  have "[p] \<parallel> [q] ;\<^sub>c [r] \<parallel> [v] = (p \<interleave> q) ;\<^sub>c (r \<interleave> v)" by (auto simp:  cnf_concurrency_def)
+  have "([p] ;\<^sub>c [r]) \<parallel> ([q] ;\<^sub>c [v]) = (p @ r) \<interleave> (q @ v)" by (auto simp: composition_cnf_def cnf_concurrency_def)
+  have "set ((p \<interleave> q) ;\<^sub>c (r \<interleave> v)) \<subseteq> set ((p @ r) \<interleave> (q @ v))"
+    by (simp add: inter1)
+  show ?thesis
+    by (simp add: \<open>([p] ;\<^sub>c [r]) \<parallel> ([q] ;\<^sub>c [v]) = (p @ r) \<interleave> (q @ v)\<close> \<open>[p] \<parallel> [q] ;\<^sub>c [r] \<parallel> [v] = (p \<interleave> q) ;\<^sub>c (r \<interleave> v)\<close> \<open>set ((p \<interleave> q) ;\<^sub>c (r \<interleave> v)) \<subseteq> set ((p @ r) \<interleave> (q @ v))\<close>)
+qed
+
+lemma prop10_4: "set ([p] \<parallel> [q] ;\<^sub>c [r] \<parallel> vs) \<subseteq> set (([p] ;\<^sub>c [r]) \<parallel> ([q] ;\<^sub>c vs))"
+proof (induction vs)
+  case Nil
+  then show ?case by (auto simp: cnf_concurrency_def composition_cnf_def)
+next
+  case (Cons v vs)
+  have "set ([p] \<parallel> [q] ;\<^sub>c [r] \<parallel> (v # vs)) = set ([p] \<parallel> [q] ;\<^sub>c [r] \<parallel> [v]) \<union> set ([p] \<parallel> [q] ;\<^sub>c [r] \<parallel> vs)"
+    apply (simp add: cnf_concurrency_def composition_cnf_def)
+    by blast
+  have "set (([p] ;\<^sub>c [r]) \<parallel> ([q] ;\<^sub>c (v # vs))) = set (([p] ;\<^sub>c [r]) \<parallel> ([q] ;\<^sub>c [v])) \<union> set (([p] ;\<^sub>c [r]) \<parallel> ([q] ;\<^sub>c vs))"
+    by (simp add: cnf_concurrency_def composition_cnf_def)
+  have "set ([p] \<parallel> [q] ;\<^sub>c [r] \<parallel> [v]) \<subseteq> set (([p] ;\<^sub>c [r]) \<parallel> ([q] ;\<^sub>c [v]))"
+    by (simp add: prop10_3_1)
+  have "set ([p] \<parallel> [q] ;\<^sub>c [r] \<parallel> vs) \<subseteq> set (([p] ;\<^sub>c [r]) \<parallel> ([q] ;\<^sub>c vs))"
+    using local.Cons by auto
+  then show "set ([p] \<parallel> [q] ;\<^sub>c [r] \<parallel> (v # vs)) \<subseteq> set (([p] ;\<^sub>c [r]) \<parallel> ([q] ;\<^sub>c (v # vs)))"
+    using \<open>set (([p] ;\<^sub>c [r]) \<parallel> ([q] ;\<^sub>c (v # vs))) = set (([p] ;\<^sub>c [r]) \<parallel> ([q] ;\<^sub>c [v])) \<union> set (([p] ;\<^sub>c [r]) \<parallel> ([q] ;\<^sub>c vs))\<close> \<open>set ([p] \<parallel> [q] ;\<^sub>c [r] \<parallel> (v # vs)) = set ([p] \<parallel> [q] ;\<^sub>c [r] \<parallel> [v]) \<union> set ([p] \<parallel> [q] ;\<^sub>c [r] \<parallel> vs)\<close> \<open>set ([p] \<parallel> [q] ;\<^sub>c [r] \<parallel> [v]) \<subseteq> set (([p] ;\<^sub>c [r]) \<parallel> ([q] ;\<^sub>c [v]))\<close> by auto
+qed
+
 lemma prop11: "set ([p] \<parallel> qs ;\<^sub>c [r]) \<subseteq> set ([p] \<parallel> (qs ;\<^sub>c [r]))"
 proof (induction qs)
   case Nil
@@ -1766,6 +1852,25 @@ next
     by (simp add: local.Cons)
   then show "set ([p] ;\<^sub>c (q # qs) \<parallel> [r]) \<subseteq> set (([p] ;\<^sub>c (q # qs)) \<parallel> [r])"
     using \<open>set (([p] ;\<^sub>c (q # qs)) \<parallel> [r]) = set (([p] ;\<^sub>c [q]) \<parallel> [r]) \<union> set (([p] ;\<^sub>c qs) \<parallel> [r])\<close> \<open>set ([p] ;\<^sub>c (q # qs) \<parallel> [r]) = set ([p] ;\<^sub>c [q] \<parallel> [r]) \<union> set ([p] ;\<^sub>c qs \<parallel> [r])\<close> \<open>set ([p] ;\<^sub>c [q] \<parallel> [r]) \<subseteq> set (([p] ;\<^sub>c [q]) \<parallel> [r])\<close> by auto
+qed
+
+lemma prop15: "set ([p] \<parallel> ([q]) ;\<^sub>c rs \<parallel> s) \<subseteq> set (([p] ;\<^sub>c rs) \<parallel> ([q] ;\<^sub>c s))"
+proof (induction rs)
+  case Nil
+  then show ?case by (auto simp: composition_cnf_def cnf_concurrency_def)
+next
+  case (Cons r rs)
+  have "set ([p] \<parallel> [q] ;\<^sub>c (r # rs) \<parallel> s) = set ([p] \<parallel> [q] ;\<^sub>c [r] \<parallel> s) \<union> set ([p] \<parallel> [q] ;\<^sub>c rs \<parallel> s)"
+    apply (simp add: composition_cnf_def cnf_concurrency_def)
+    by (simp add: complete_lattice_class.SUP_sup_distrib)
+  have "set (([p] ;\<^sub>c (r # rs)) \<parallel> ([q] ;\<^sub>c s)) = set (([p] ;\<^sub>c [r]) \<parallel> ([q] ;\<^sub>c s)) \<union> set (([p] ;\<^sub>c rs) \<parallel> ([q] ;\<^sub>c s))"
+    by (simp add: composition_cnf_def cnf_concurrency_def)
+  have "set ([p] \<parallel> [q] ;\<^sub>c [r] \<parallel> s) \<subseteq> set (([p] ;\<^sub>c [r]) \<parallel> ([q] ;\<^sub>c s))"
+    by (simp add: prop10_4)
+  have "set ([p] \<parallel> [q] ;\<^sub>c rs \<parallel> s) \<subseteq> set (([p] ;\<^sub>c rs) \<parallel> ([q] ;\<^sub>c s))"
+    by (simp add: local.Cons)
+  then show "set ([p] \<parallel> [q] ;\<^sub>c (r # rs) \<parallel> s) \<subseteq> set (([p] ;\<^sub>c (r # rs)) \<parallel> ([q] ;\<^sub>c s))"
+    using \<open>set (([p] ;\<^sub>c (r # rs)) \<parallel> ([q] ;\<^sub>c s)) = set (([p] ;\<^sub>c [r]) \<parallel> ([q] ;\<^sub>c s)) \<union> set (([p] ;\<^sub>c rs) \<parallel> ([q] ;\<^sub>c s))\<close> \<open>set ([p] \<parallel> [q] ;\<^sub>c (r # rs) \<parallel> s) = set ([p] \<parallel> [q] ;\<^sub>c [r] \<parallel> s) \<union> set ([p] \<parallel> [q] ;\<^sub>c rs \<parallel> s)\<close> \<open>set ([p] \<parallel> [q] ;\<^sub>c [r] \<parallel> s) \<subseteq> set (([p] ;\<^sub>c [r]) \<parallel> ([q] ;\<^sub>c s))\<close> by auto
 qed
 
 
@@ -1841,6 +1946,24 @@ next
     by (simp add: local.Cons)
   then show "set ([p] ;\<^sub>c q \<parallel> (r # rs)) \<subseteq> set (([p] ;\<^sub>c q) \<parallel> (r # rs))"
     using \<open>set (([p] ;\<^sub>c q) \<parallel> (r # rs)) = set (([p] ;\<^sub>c q) \<parallel> [r]) \<union> set (([p] ;\<^sub>c q) \<parallel> rs)\<close> \<open>set ([p] ;\<^sub>c q \<parallel> (r # rs)) = set ([p] ;\<^sub>c q \<parallel> [r]) \<union> set ([p] ;\<^sub>c q \<parallel> rs)\<close> \<open>set ([p] ;\<^sub>c q \<parallel> [r]) \<subseteq> set (([p] ;\<^sub>c q) \<parallel> [r])\<close> by auto
+qed
+
+lemma subset16: "set ([p] \<parallel> qs ;\<^sub>c r \<parallel> s) \<subseteq> set (([p] ;\<^sub>c r) \<parallel> (qs ;\<^sub>c s))"
+proof (induction qs)
+  case Nil
+  then show ?case by (auto simp: composition_cnf_def cnf_concurrency_def)
+next
+  case (Cons q qs)
+  have "set ([p] \<parallel> (q # qs) ;\<^sub>c r \<parallel> s) = set ([p] \<parallel> ([q]) ;\<^sub>c r \<parallel> s) \<union> set ([p] \<parallel> qs ;\<^sub>c r \<parallel> s)"
+    by (auto simp: composition_cnf_def cnf_concurrency_def)
+  have "set (([p] ;\<^sub>c r) \<parallel> ((q # qs) ;\<^sub>c s)) = set (([p] ;\<^sub>c r) \<parallel> ([q] ;\<^sub>c s)) \<union> set (([p] ;\<^sub>c r) \<parallel> ((qs) ;\<^sub>c s))"
+    by (auto simp: composition_cnf_def cnf_concurrency_def)
+  have "set ([p] \<parallel> ([q]) ;\<^sub>c r \<parallel> s) \<subseteq> set (([p] ;\<^sub>c r) \<parallel> ([q] ;\<^sub>c s))"
+    by (simp add: prop15)
+  have "set ([p] \<parallel> qs ;\<^sub>c r \<parallel> s) \<subseteq> set (([p] ;\<^sub>c r) \<parallel> ((qs) ;\<^sub>c s))"
+    by (simp add: local.Cons)
+  then show "set ([p] \<parallel> (q # qs) ;\<^sub>c r \<parallel> s) \<subseteq> set (([p] ;\<^sub>c r) \<parallel> ((q # qs) ;\<^sub>c s))"
+    using \<open>set (([p] ;\<^sub>c r) \<parallel> ((q # qs) ;\<^sub>c s)) = set (([p] ;\<^sub>c r) \<parallel> ([q] ;\<^sub>c s)) \<union> set (([p] ;\<^sub>c r) \<parallel> (qs ;\<^sub>c s))\<close> \<open>set ([p] \<parallel> (q # qs) ;\<^sub>c r \<parallel> s) = set ([p] \<parallel> [q] ;\<^sub>c r \<parallel> s) \<union> set ([p] \<parallel> qs ;\<^sub>c r \<parallel> s)\<close> \<open>set ([p] \<parallel> [q] ;\<^sub>c r \<parallel> s) \<subseteq> set (([p] ;\<^sub>c r) \<parallel> ([q] ;\<^sub>c s))\<close> by auto
 qed
 
 theorem Conc_composeright_1: "set ((p \<parallel> q) ;\<^sub>c rs) \<subseteq> set (p \<parallel> (q ;\<^sub>c rs))"
@@ -1949,5 +2072,928 @@ theorem Conc_composegeneral: "set (([p] ;\<^sub>c [u]) \<parallel> ([q] ;\<^sub>
   oops
 theorem Conc_composegeneral: "set ((p ;\<^sub>c q) \<parallel> (u ;\<^sub>c v)) \<subseteq> set ((p ;\<^sub>c u) \<parallel> (q ;\<^sub>c v))" \<comment> \<open>Conc_composegeneral\<close>
   oops
+
+theorem Conc_composegeneral_1: "set ((ps \<parallel> q) ;\<^sub>c (r \<parallel> s)) \<subseteq> set ((ps ;\<^sub>c r) \<parallel> (q ;\<^sub>c s))"
+proof (induction ps)
+  case Nil
+  then show ?case
+    by (auto simp: composition_cnf_def cnf_concurrency_def)
+next
+  case (Cons p ps)
+  have "set ((p # ps) \<parallel> q ;\<^sub>c r \<parallel> s) = set ([p] \<parallel> q ;\<^sub>c r \<parallel> s) \<union> set ((ps) \<parallel> q ;\<^sub>c r \<parallel> s)"
+    by (auto simp: composition_cnf_def cnf_concurrency_def)
+  have "set (((p # ps) ;\<^sub>c r) \<parallel> (q ;\<^sub>c s)) = set (([p] ;\<^sub>c r) \<parallel> (q ;\<^sub>c s)) \<union> set (((ps) ;\<^sub>c r) \<parallel> (q ;\<^sub>c s))"
+    by (auto simp: composition_cnf_def cnf_concurrency_def)
+  have "set ([p] \<parallel> q ;\<^sub>c r \<parallel> s) \<subseteq> set (([p] ;\<^sub>c r) \<parallel> (q ;\<^sub>c s))"
+    by (simp add: subset16)
+  have "set ((ps) \<parallel> q ;\<^sub>c r \<parallel> s) \<subseteq> set (((ps) ;\<^sub>c r) \<parallel> (q ;\<^sub>c s))"
+    using local.Cons by auto
+  then show "set ((p # ps) \<parallel> q ;\<^sub>c r \<parallel> s) \<subseteq> set (((p # ps) ;\<^sub>c r) \<parallel> (q ;\<^sub>c s))"
+    using \<open>set (((p # ps) ;\<^sub>c r) \<parallel> (q ;\<^sub>c s)) = set (([p] ;\<^sub>c r) \<parallel> (q ;\<^sub>c s)) \<union> set ((ps ;\<^sub>c r) \<parallel> (q ;\<^sub>c s))\<close> \<open>set ((p # ps) \<parallel> q ;\<^sub>c r \<parallel> s) = set ([p] \<parallel> q ;\<^sub>c r \<parallel> s) \<union> set (ps \<parallel> q ;\<^sub>c r \<parallel> s)\<close> \<open>set ([p] \<parallel> q ;\<^sub>c r \<parallel> s) \<subseteq> set (([p] ;\<^sub>c r) \<parallel> (q ;\<^sub>c s))\<close> by auto
+qed
+
+theorem Conc_composegeneral: "evaluate ((p \<parallel> q) ;\<^sub>c (r \<parallel> s)) C \<preceq>\<^sub>p evaluate ((p ;\<^sub>c r) \<parallel> (q ;\<^sub>c s)) C" \<comment> \<open>Conc_composegeneral\<close>
+  by (simp add: Conc_composegeneral_1 eval_subprogram12)
+
+lemma "foldl (+) (b::nat) xs = b + foldl (+) 0 xs" apply (induction xs) apply auto
+  by (simp add: simp_2)
+
+fun cnf_size :: "'a CNF \<Rightarrow> nat" where
+  "cnf_size [] = 0" |
+  "cnf_size (x#xs) = length x + cnf_size xs + 1"
+
+
+function cnf_concurrency2 :: "'a CNF \<Rightarrow> 'a CNF \<Rightarrow> 'a set \<Rightarrow> 'a Program" where
+  "cnf_concurrency2 [] ys C = Fail {}" |
+  "cnf_concurrency2 xs [] C = Fail {}" |
+  "cnf_concurrency2 (x#xs) (y#ys) C = 
+     (case (xs , ys) of
+        ([], []) \<Rightarrow> (case (x, y) of 
+          ([], []) \<Rightarrow> Skip C |
+          ([a], [b]) \<Rightarrow> a;b \<union>\<^sub>p b;a |
+          ([], bs) \<Rightarrow> evaluate [bs] C |
+          (as, []) \<Rightarrow> evaluate [as] C |
+          (a#as, b#bs) \<Rightarrow> a; (cnf_concurrency2 [as] [b#bs] C) \<union>\<^sub>p b; (cnf_concurrency2 [a#as] [bs] C)) |
+        (f#fs, []) \<Rightarrow> cnf_concurrency2 [x] [y] C \<union>\<^sub>p cnf_concurrency2 (f#fs) [y] C |
+        ([], g#gs) \<Rightarrow> cnf_concurrency2 [x] [y] C \<union>\<^sub>p cnf_concurrency2 [x] (g#gs) C |
+        (f#fs, g#gs) \<Rightarrow> cnf_concurrency2 [x] (y#g#gs) C \<union>\<^sub>p cnf_concurrency2 (f#fs) (y#g#gs) C
+  )"
+  by pat_completeness auto
+termination cnf_concurrency2
+  apply (relation "measure (\<lambda>(xs, ys, _). cnf_size xs + cnf_size ys)")
+  by auto
+declare cnf_concurrency2.simps [simp del]
+
+theorem cnf_concurrency2_simp1 [simp]: "cnf_concurrency2 [] ys C = Fail {}"
+  by (simp add: cnf_concurrency2.simps(1))
+
+theorem cnf_concurrency2_simp2 [simp]: "cnf_concurrency2 xs [] C = Fail {}"
+  by (simp add: cnf_concurrency2.simps(2))
+
+theorem cnf_concurrency2_simp3 [simp]: "cnf_concurrency2 [] [] C = Fail {}"
+  by (simp)
+
+theorem cnf_concurrency2_simp4 [simp]: "cnf_concurrency2 [[]] [[]] C = Skip C"
+  using cnf_concurrency2.simps(3)
+  by (smt (verit) case_prod_conv list.simps(4))
+
+theorem cnf_concurrency2_simp5 [simp]: "cnf_concurrency2 [[a]] [[b]] C = a;b \<union>\<^sub>p b;a"
+  using cnf_concurrency2.simps(3)
+  by (smt (verit, del_insts) case_prod_conv list.simps(4) list.simps(5))
+
+theorem cnf_concurrency2_simp6 [simp]: "cnf_concurrency2 [[a]] [[]] C = a"
+proof -
+  have "cnf_concurrency2 [[a]] [[]] C = evaluate [[a]] C"
+  using cnf_concurrency2.simps(3)
+  by (smt (verit, del_insts) case_prod_conv list.simps(4) list.simps(5))
+  have "evaluate [[a]] C = a" by (auto simp: evaluate_def)
+  show ?thesis
+    by (simp add: \<open>cnf_concurrency2 [[a]] [[]] C = evaluate [[a]] C\<close> \<open>evaluate [[a]] C = a\<close>)
+qed
+
+theorem cnf_concurrency2_simp7 [simp]: "cnf_concurrency2 [[]] [[b]] C = b"
+proof -
+  have "cnf_concurrency2 [[]] [[b]] C = evaluate [[b]] C"
+  using cnf_concurrency2.simps(3)
+  by (smt (verit, del_insts) case_prod_conv list.simps(4) list.simps(5))
+  have "evaluate [[b]] C = b" by (auto simp: evaluate_def)
+  show ?thesis
+    by (simp add: \<open>cnf_concurrency2 [[]] [[b]] C = evaluate [[b]] C\<close> \<open>evaluate [[b]] C = b\<close>)
+qed
+
+theorem cnf_concurrency2_simp8 [simp]: "cnf_concurrency2 [a#as] [b#bs] C = a;(cnf_concurrency2 [as] [b#bs] C) \<union>\<^sub>p (b;cnf_concurrency2 [a#as] [bs] C)"
+  using cnf_concurrency2.simps(3) case_prod_conv cnf_concurrency2_simp7 list.exhaust list.simps(4) list.simps(5)
+  by (smt (z3) neq_Nil_conv)
+
+theorem cnf_concurrency2_simp9 [simp]: "cnf_concurrency2 [x, xx] [y] C = cnf_concurrency2 [x] [y] C \<union>\<^sub>p cnf_concurrency2 [xx] [y] C"
+    by (simp add: cnf_concurrency2.simps(3))
+
+theorem cnf_concurrency2_simp10 [simp]: "cnf_concurrency2 [x] [y, yy] C = cnf_concurrency2 [x] [y] C \<union>\<^sub>p cnf_concurrency2 [x] [yy] C"
+    by (simp add: cnf_concurrency2.simps(3))
+
+theorem cnf_concurrency2_simp11 [simp]: "cnf_concurrency2 (x#xx#xs) [y] C = cnf_concurrency2 [x] [y] C \<union>\<^sub>p cnf_concurrency2 (xx#xs) [y] C"
+    by (simp add: cnf_concurrency2.simps(3))
+
+theorem cnf_concurrency2_simp12 [simp]: "cnf_concurrency2 [y] (x#xx#xs) C = cnf_concurrency2 [y] [x] C \<union>\<^sub>p cnf_concurrency2 [y] (xx#xs) C"
+    by (simp add: cnf_concurrency2.simps(3))
+
+theorem cnf_concurrency2_simp13 [simp]: "cnf_concurrency2 [[]] [y # ys] C = evaluate [y # ys] C" 
+    by (simp add: cnf_concurrency2.simps(3))
+
+theorem cnf_concurrency2_simp14 [simp]: "cnf_concurrency2 [y # yy # ys] [[]]  C = evaluate [y # yy # ys] C" 
+  using cnf_concurrency2.simps(3) case_prod_conv cnf_concurrency2_simp7 list.exhaust list.simps(4) list.simps(5)
+  apply auto
+  by (simp add: cnf_concurrency2.simps(3) evaluate_def)
+
+theorem cnf_concurrency2_simp15 [simp]: "cnf_concurrency2 [y # ys] [[]]  C = evaluate [y # ys] C" 
+  using cnf_concurrency2.simps(3) case_prod_conv cnf_concurrency2_simp7 list.exhaust list.simps(4) list.simps(5)
+  apply (cases "ys")
+    apply (simp add: cnf_concurrency2.simps(3) evaluate_def)
+  by (simp add:)
+
+theorem cnf_concurrenc2_simp16 [simp]: "cnf_concurrency2 (y1#y2#ys) (x1#x2#xs) C = cnf_concurrency2 [y1] (x1#x2#xs) C \<union>\<^sub>p cnf_concurrency2 (y2#ys) (x1#x2#xs) C"
+  using cnf_concurrency2.simps(3)[of y1 "y2#ys" x1 "x2#xs"] case_prod_conv cnf_concurrency2_simp7 list.exhaust list.simps(4) list.simps(5)
+  by (auto)
+
+theorem cnf_concurrency2_simp17 [simp]: "cnf_concurrency2 [[]] [ys] C = evaluate [ys] C" 
+  using cnf_concurrency2.simps(3)[of "[]" "[]" "ys" "[]" C]
+  apply auto
+  by (smt (verit) Choice.simps(2) Concat.elims cnf_concurrency2_simp13 evaluate_def list.simps(4) list.simps(8) list.simps(9))
+
+theorem cnf_concurrency2_simp18 [simp]: "cnf_concurrency2 [xs] [[]] C = evaluate [xs] C" 
+  using cnf_concurrency2.simps(3)[of "xs" "[]" "[]" "[]" C]
+  apply auto
+  by (metis (no_types, lifting) cnf_concurrency2_simp15 cnf_concurrency2_simp17 permutations.cases)
+
+theorem cnf_concurrency2_simp19 [simp]: "cnf_concurrency2 xs [[]] C = evaluate xs C"
+proof (induction xs)
+  case Nil
+  then show ?case by (auto simp: evaluate_def)
+next
+  case (Cons x xs)
+  then show ?case 
+  using cnf_concurrency2.simps(3)[of x xs "[]" "[]" C] apply auto
+  by (metis (no_types, lifting) cnf_concurrency2_simp11 cnf_concurrency2_simp18 cnf_size.cases concat_prop3)
+qed
+
+theorem cnf_prop1: "cnf_concurrency2 [[x]] [[y]] C = evaluate ([x] \<interleave> [y]) C"
+  by (auto simp: evaluate_def) 
+
+theorem "is_rounded a \<Longrightarrow> (a;b) \<union>\<^sub>p (a;c) = a;(b \<union>\<^sub>p c)"
+  apply (simp add: is_rounded_def composition_def choice_def corestrict_r_def S_def restr_post_def restrict_r_def relcomp_unfold Field_def) 
+  by auto
+
+
+theorem cnf2_prop: "cnf_feasible ([y]#ys) \<Longrightarrow> complete_cnf_state ([y]#ys) \<subseteq> C \<Longrightarrow> \<Union>\<^sub>p (map ((\<lambda>xs. Concat xs C) \<circ> (#) y) (ys)) \<equiv>\<^sub>p y ; \<Union>\<^sub>p (map (\<lambda>xs. Concat xs C) (ys))" 
+proof (induction ys)
+  case Nil
+  then show ?case apply auto
+  apply (simp add: equiv_is_symetric fail_compose_r) done
+next
+  case (Cons a ys)
+  have "is_feasible y"
+    using Cons.prems(1) by auto
+  have "S y \<subseteq> C"
+    by (metis Cons.prems(2) cnf_concurrency2_simp15 cnf_concurrency2_simp6 length_prop_1 member_rec(1) order.partial_preordering_axioms partial_preordering_def state_prop10 state_prop11 state_prop6)
+  have "y ; Skip C \<equiv>\<^sub>p y"
+    by (simp add: Big_choice.skip_prop \<open>S y \<subseteq> C\<close> \<open>is_feasible y\<close>)
+  have "complete_cnf_state ([y] # ys) \<subseteq> C"
+    by (metis (no_types, lifting) Cons.prems(2) cnf_choice2 dual_order.trans state_prop12 subset3)
+  have "cnf_feasible ([y] # ys)"
+    using Cons.prems(1) by auto
+  have l1: "\<Union>\<^sub>p (map ((\<lambda>xs. Concat xs C) \<circ> (#) y) (a # ys)) \<equiv>\<^sub>p \<Union>\<^sub>p (map ((\<lambda>xs. Concat xs C) \<circ> (#) y) [a]) \<union>\<^sub>p \<Union>\<^sub>p (map ((\<lambda>xs. Concat xs C) \<circ> (#) y) ys)"
+    apply auto
+    by (metis Choice.simps(1) Choice.simps(2) Choice_prop_1_2 equals_equiv_relation_3 equiv_is_symetric fail_choice_r)
+  have l2: "... = Concat (y # a) C \<union>\<^sub>p \<Union>\<^sub>p (map ((\<lambda>xs. Concat xs C) \<circ> (#) y) ys)" by auto
+  have l3: "... \<equiv>\<^sub>p Concat (y # a) C \<union>\<^sub>p (y ; \<Union>\<^sub>p (map (\<lambda>xs. Concat xs C) ys))" using Cons apply auto
+    by (simp add: Cons.IH \<open>complete_cnf_state ([y] # ys) \<subseteq> C\<close> choice_equiv equiv_is_reflexive)
+  have "\<Union>\<^sub>p (map ((\<lambda>xs. Concat xs C) \<circ> (#) y) (a # ys)) \<equiv>\<^sub>p Concat (y # a) C \<union>\<^sub>p (y ; \<Union>\<^sub>p (map (\<lambda>xs. Concat xs C) ys))" using l1 l2 l3 equiv_is_transitive by auto
+  show ?case
+  proof (cases "a=[]")
+    case True
+    have "\<Union>\<^sub>p (map ((\<lambda>xs. Concat xs C) \<circ> (#) y) (a # ys)) = \<Union>\<^sub>p (map ((\<lambda>xs. Concat xs C) \<circ> (#) y) ([] # ys))"
+      by (simp add: True)
+    then have l4: "Concat (y # a) C \<union>\<^sub>p (y ; \<Union>\<^sub>p (map (\<lambda>xs. Concat xs C) ys)) = Concat [y] C \<union>\<^sub>p (y ; \<Union>\<^sub>p (map (\<lambda>xs. Concat xs C) ys))"
+      by (simp add: True)
+    have l5: "... = y \<union>\<^sub>p (y ; \<Union>\<^sub>p (map (\<lambda>xs. Concat xs C) ys))" by auto
+    have l6: "... \<equiv>\<^sub>p (y ; Skip C) \<union>\<^sub>p (y ; \<Union>\<^sub>p (map (\<lambda>xs. Concat xs C) ys))" 
+      using \<open>y ; Skip C \<equiv>\<^sub>p y\<close>
+      using choice_equiv equiv_is_reflexive equiv_is_symetric by blast
+    have l7: "... \<equiv>\<^sub>p (y ; (Skip C \<union>\<^sub>p \<Union>\<^sub>p (map (\<lambda>xs. Concat xs C) ys)))" by (simp add: compose_distrib1_3 equiv_is_symetric) 
+    have l8: "... = y ; \<Union>\<^sub>p (Skip C # map (\<lambda>xs. Concat xs C) ys)"
+      by (metis Choice.simps(2) Choice_prop_1_2 Choice_prop_22 \<open>S y \<subseteq> C\<close> choice_idem_2 skip_prop_10 sup.absorb_iff1)
+    have "\<Union>\<^sub>p (map ((\<lambda>xs. Concat xs C) \<circ> (#) y) ([] # ys)) \<equiv>\<^sub>p y ; \<Union>\<^sub>p (map (\<lambda>xs. Concat xs C) ([] # ys))"
+      by (smt (verit, best) Concat.simps(1) True \<open>\<Union>\<^sub>p (map ((\<lambda>xs. Concat xs C) \<circ> (#) y) (a # ys)) \<equiv>\<^sub>p Concat (y # a) C \<union>\<^sub>p y ; \<Union>\<^sub>p (map (\<lambda>xs. Concat xs C) ys)\<close> equiv_is_transitive list.simps(9) local.l5 local.l6 local.l7 local.l8)
+    then show ?thesis
+      using True by blast
+  next
+    case False
+    have "Concat (y # a) C \<union>\<^sub>p (y ; \<Union>\<^sub>p (map (\<lambda>xs. Concat xs C) ys)) = y ; Concat (a) C \<union>\<^sub>p (y ; \<Union>\<^sub>p (map (\<lambda>xs. Concat xs C) ys))"
+      by (simp add: Concat_prop_10 False)
+    have "... \<equiv>\<^sub>p y ; ((Concat (a) C) \<union>\<^sub>p \<Union>\<^sub>p (map (\<lambda>xs. Concat xs C) ys))"
+      by (simp add: compose_distrib1_3 equiv_is_symetric)
+    have "... \<equiv>\<^sub>p y ; \<Union>\<^sub>p (map (\<lambda>xs. Concat xs C) (a#ys))" apply (cases "ys=[]") apply auto
+      apply (simp add: composition_equiv equals_equiv_relation_3 fail_choice_l)
+      by (simp add: Choice_prop_1_2 equals_equiv_relation_3)
+    then show ?thesis
+      by (smt (verit, best) \<open>Concat (y # a) C \<union>\<^sub>p \<Union>\<^sub>p (map ((\<lambda>xs. Concat xs C) \<circ> (#) y) ys) \<equiv>\<^sub>p Concat (y # a) C \<union>\<^sub>p y ; \<Union>\<^sub>p (map (\<lambda>xs. Concat xs C) ys)\<close> \<open>Concat (y # a) C \<union>\<^sub>p y ; \<Union>\<^sub>p (map (\<lambda>xs. Concat xs C) ys) = y ; Concat a C \<union>\<^sub>p y ; \<Union>\<^sub>p (map (\<lambda>xs. Concat xs C) ys)\<close> \<open>\<Union>\<^sub>p (map ((\<lambda>xs. Concat xs C) \<circ> (#) y) (a # ys)) \<equiv>\<^sub>p \<Union>\<^sub>p (map ((\<lambda>xs. Concat xs C) \<circ> (#) y) [a]) \<union>\<^sub>p \<Union>\<^sub>p (map ((\<lambda>xs. Concat xs C) \<circ> (#) y) ys)\<close> \<open>\<Union>\<^sub>p (map ((\<lambda>xs. Concat xs C) \<circ> (#) y) [a]) \<union>\<^sub>p \<Union>\<^sub>p (map ((\<lambda>xs. Concat xs C) \<circ> (#) y) ys) = Concat (y # a) C \<union>\<^sub>p \<Union>\<^sub>p (map ((\<lambda>xs. Concat xs C) \<circ> (#) y) ys)\<close> \<open>y ; Concat a C \<union>\<^sub>p y ; \<Union>\<^sub>p (map (\<lambda>xs. Concat xs C) ys) \<equiv>\<^sub>p y ; (Concat a C \<union>\<^sub>p \<Union>\<^sub>p (map (\<lambda>xs. Concat xs C) ys))\<close> equiv_is_transitive)
+  qed
+qed 
+
+theorem cnf2_prop2: "cnf_feasible xs \<Longrightarrow> is_feasible x \<Longrightarrow> cnf_feasible (map ((#) x) (xs))"
+proof (induction xs)
+  case Nil
+  then show ?case by auto
+next
+  case (Cons a xs)
+  then have "cnf_feasible xs"
+    by simp
+  then have "cnf_feasible (map ((#) x) xs)" using Cons(3) Cons(1) by auto
+  have "map ((#) x) (a # xs) = (x#a) # map ((#) x) xs" by auto
+  have "all_feasible (x#a)"
+    using Cons.prems(1) Cons.prems(2) by auto
+  then show ?case
+    by (simp add: \<open>cnf_feasible (map ((#) x) xs)\<close>)
+qed
+
+theorem cnf2_prop3: "cnf_feasible xs \<Longrightarrow> cnf_feasible ys \<Longrightarrow> cnf_feasible (xs@ys)"
+  apply (induction xs) by auto
+
+theorem cnf2_prop4: "all_feasible (xs@ys) \<Longrightarrow> cnf_feasible (xs \<interleave> ys)"
+proof (induction xs arbitrary: ys)
+  case Nil
+  then show ?case by auto
+next
+  case (Cons x xs)
+  moreover have "cnf_feasible (xs \<interleave> ys)"
+    using Cons.IH Cons.prems by force
+  ultimately show ?case
+  proof (induction ys)
+    case Nil
+    then show ?case by auto
+  next
+    case (Cons y ys)
+    have "cnf_feasible ((x # xs) \<interleave> ys)"
+      by (metis Cons.IH Cons.prems(1) Cons.prems(2) all_feasible.simps(2) feas_prop1 feas_prop2 feas_prop8)
+    have "cnf_feasible (xs \<interleave> (y#ys))"
+      by (simp add: Cons.prems(3))
+    have "cnf_feasible (map ((#) y) ((x # xs) \<interleave> ys))"
+      using Cons.prems(2) \<open>cnf_feasible ((x # xs) \<interleave> ys)\<close> all_feasible.simps(2) cnf2_prop2 feas_prop2 by blast
+    have "cnf_feasible (map ((#) x) (xs \<interleave> (y # ys)) @ map ((#) y) ((x # xs) \<interleave> ys))"
+      using Cons.prems(2) Cons.prems(3) \<open>cnf_feasible (map ((#) y) ((x # xs) \<interleave> ys))\<close> all_feasible.simps(2) cnf2_prop2 cnf2_prop3 feas_prop1 by blast
+    then show ?case
+      by simp
+  qed
+qed
+
+theorem cnf2_prop5: "xs \<noteq> [] \<Longrightarrow> complete_cnf_state (map ((#) x) xs) = S x \<union> complete_cnf_state xs"
+proof (induction xs)
+  case Nil
+  then show ?case by auto
+next
+  case (Cons y xs)
+  then show "complete_cnf_state (map ((#) x) (y # xs)) = S x \<union> complete_cnf_state (y # xs)"
+  proof (cases "xs=[]")
+    case True
+    then show ?thesis apply (auto simp: complete_cnf_state_def complete_state_def)
+      apply (metis Un_iff complete_state_prop_3 complete_state_prop_4)
+      apply (metis Un_iff complete_state_prop_3 complete_state_prop_4)
+      by (metis Un_iff complete_state_prop_3 complete_state_prop_4)
+  next
+    case False
+    have "complete_cnf_state (map ((#) x) xs) = S x \<union> complete_cnf_state xs"
+      by (simp add: Cons.IH False)
+    have "complete_cnf_state (map ((#) x) (y # xs)) = complete_cnf_state (map ((#) x) [y]) \<union> complete_cnf_state (map ((#) x) xs)"
+      by (auto simp: complete_cnf_state_def)
+    have "complete_cnf_state (map ((#) x) [y]) = S x \<union> complete_state y" apply (auto simp: complete_cnf_state_def complete_state_def)
+      apply (metis Un_iff complete_state_prop_3 complete_state_prop_4)
+      apply (metis Un_iff complete_state_prop_3 complete_state_prop_4)
+      by (metis Un_iff complete_state_prop_3 complete_state_prop_4)
+    have "complete_cnf_state (map ((#) x) [y]) \<union> complete_cnf_state (map ((#) x) xs) = S x \<union> complete_state y \<union> complete_cnf_state (map ((#) x) xs)"
+      using \<open>complete_cnf_state (map ((#) x) [y]) = S x \<union> complete_state y\<close> by auto
+    have "S x \<union> complete_state y \<union> complete_cnf_state (map ((#) x) xs) = S x \<union> complete_state y \<union> S x \<union> complete_cnf_state xs"
+      using \<open>complete_cnf_state (map ((#) x) xs) = S x \<union> complete_cnf_state xs\<close> by auto 
+    have "... = S x \<union> S x \<union> complete_state y \<union> complete_cnf_state xs" by auto
+    have "... = S x \<union> complete_state y \<union> complete_cnf_state xs" by auto
+    have "... = S x \<union> complete_cnf_state (y#xs)" by (auto simp: complete_cnf_state_def)
+    then show ?thesis
+      using \<open>S x \<union> S x \<union> complete_state y \<union> complete_cnf_state xs = S x \<union> complete_state y \<union> complete_cnf_state xs\<close> \<open>S x \<union> complete_state y \<union> S x \<union> complete_cnf_state xs = S x \<union> S x \<union> complete_state y \<union> complete_cnf_state xs\<close> \<open>S x \<union> complete_state y \<union> complete_cnf_state (map ((#) x) xs) = S x \<union> complete_state y \<union> S x \<union> complete_cnf_state xs\<close> \<open>complete_cnf_state (map ((#) x) (y # xs)) = complete_cnf_state (map ((#) x) [y]) \<union> complete_cnf_state (map ((#) x) xs)\<close> \<open>complete_cnf_state (map ((#) x) [y]) \<union> complete_cnf_state (map ((#) x) xs) = S x \<union> complete_state y \<union> complete_cnf_state (map ((#) x) xs)\<close> by presburger
+  qed
+qed 
+
+theorem cnf2_prop6: "complete_cnf_state xs \<union> complete_cnf_state ys = complete_cnf_state (xs@ys)"
+  apply (induction xs) by (auto simp: complete_cnf_state_def)
+
+theorem cnf2_prop7: "complete_state xs \<union> complete_state ys = complete_cnf_state (xs \<interleave> ys)"
+proof (induction xs arbitrary: ys)
+  case Nil
+  then show ?case by (auto simp:  complete_state_def complete_cnf_state_def)
+next
+  case Cons1: (Cons x xs)
+  then have "complete_state xs \<union> complete_state ys = complete_cnf_state (xs \<interleave> ys)" by simp
+  then show ?case using Cons1
+  proof (induction ys)
+    case Nil
+    then show ?case by (auto simp:  complete_state_def complete_cnf_state_def)
+  next
+    case (Cons y ys)
+    have "complete_cnf_state (map ((#) x) (xs \<interleave> (y # ys)) @ map ((#) y) ((x # xs) \<interleave> ys)) = 
+          complete_cnf_state (map ((#) x) (xs \<interleave> (y # ys))) \<union> complete_cnf_state (map ((#) y) ((x # xs) \<interleave> ys))"
+      by (simp add: cnf2_prop6)
+    have "complete_state (x # xs) \<union> complete_state ys = complete_cnf_state ((x # xs) \<interleave> ys)"
+      by (simp add: Cons.IH Cons1)
+    have "complete_cnf_state (map ((#) x) (xs \<interleave> (y # ys))) = S x \<union> complete_cnf_state (xs \<interleave> (y # ys))"
+      by (metis append_is_Nil_conv cnf2_prop5 interleav_prop list.discI transpose.simps(1) transpose_empty)
+    have "... = S x \<union> complete_state xs \<union> complete_state (y # ys)"
+      using Cons.prems(1) by blast
+    have "... = complete_state (x # xs) \<union> complete_state (y # ys)"
+      by (simp add: complete_state_prop sup_commute)
+    have "complete_cnf_state (map ((#) y) ((x # xs) \<interleave> ys)) = S y \<union> complete_cnf_state ((x # xs) \<interleave> ys)"
+      by (metis append_is_Nil_conv cnf2_prop5 interleav_prop list.discI transpose.simps(1) transpose_empty)
+    have "... = S y \<union> complete_state (x # xs) \<union> complete_state ys"
+      using \<open>complete_state (x # xs) \<union> complete_state ys = complete_cnf_state ((x # xs) \<interleave> ys)\<close> by auto
+    have "... = complete_state (x # xs) \<union> complete_state (y # ys)"
+      by (simp add: complete_state_prop sup_commute sup_left_commute)
+    then show ?case apply simp
+      by (simp add: \<open>S x \<union> complete_cnf_state (xs \<interleave> (y # ys)) = S x \<union> complete_state xs \<union> complete_state (y # ys)\<close> \<open>S x \<union> complete_state xs \<union> complete_state (y # ys) = complete_state (x # xs) \<union> complete_state (y # ys)\<close> \<open>S y \<union> complete_cnf_state ((x # xs) \<interleave> ys) = S y \<union> complete_state (x # xs) \<union> complete_state ys\<close> \<open>complete_cnf_state (map ((#) x) (xs \<interleave> (y # ys)) @ map ((#) y) ((x # xs) \<interleave> ys)) = complete_cnf_state (map ((#) x) (xs \<interleave> (y # ys))) \<union> complete_cnf_state (map ((#) y) ((x # xs) \<interleave> ys))\<close> \<open>complete_cnf_state (map ((#) x) (xs \<interleave> (y # ys))) = S x \<union> complete_cnf_state (xs \<interleave> (y # ys))\<close> \<open>complete_cnf_state (map ((#) y) ((x # xs) \<interleave> ys)) = S y \<union> complete_cnf_state ((x # xs) \<interleave> ys)\<close>)
+  qed
+qed
+
+theorem cnf2_prop8: "S y \<subseteq> C \<Longrightarrow> is_feasible y \<Longrightarrow> \<Union>\<^sub>p (map ((\<lambda>xs. Concat xs C) \<circ> (#) y) ys) \<equiv>\<^sub>p \<Union>\<^sub>p (map (\<lambda>xs. y ; Concat xs C) ys)"
+proof (induction ys)
+  case Nil
+  then show ?case
+    by (simp add: equals_equiv_relation_3)
+next
+  case (Cons a ys)
+  have "is_feasible y"
+    using Cons.prems(2) by auto
+  show "\<Union>\<^sub>p (map ((\<lambda>xs. Concat xs C) \<circ> (#) y) (a # ys)) \<equiv>\<^sub>p \<Union>\<^sub>p (map (\<lambda>xs. y ; Concat xs C) (a # ys))"
+  proof (cases "ys=[]")
+    case True
+    then show ?thesis apply auto
+      by (metis Big_choice.skip_prop Concat.simps(1) Concat.simps(2) Concat_prop_10 \<open>S y \<subseteq> C\<close> \<open>is_feasible y\<close> equiv_is_reflexive equiv_is_symetric)
+  next
+    case False
+    then have "\<Union>\<^sub>p (map ((\<lambda>xs. Concat xs C) \<circ> (#) y) (a # ys)) = \<Union>\<^sub>p (Concat (y # a) C # map ((\<lambda>xs. Concat xs C) \<circ> (#) y) ys)" by auto
+    have "... = Concat (y # a) C \<union>\<^sub>p \<Union>\<^sub>p (map ((\<lambda>xs. Concat xs C) \<circ> (#) y) ys)"
+      by (simp add: Choice_prop_1_2 False)
+    have "... \<equiv>\<^sub>p Concat (y # a) C \<union>\<^sub>p  \<Union>\<^sub>p (map (\<lambda>xs. y ; Concat xs C) ys)"
+      using Cons.IH Cons.prems(1) Cons.prems(2) choice_equiv equals_equiv_relation_3 by blast
+    have "... \<equiv>\<^sub>p y ; Concat a C \<union>\<^sub>p  \<Union>\<^sub>p (map (\<lambda>xs. y ; Concat xs C) ys)"
+      by (metis Big_choice.skip_prop Concat.simps(1) Concat.simps(2) Concat_prop_10 \<open>S y \<subseteq> C\<close> \<open>is_feasible y\<close> choice_equiv equiv_is_reflexive equiv_is_symetric)
+    have "... \<equiv>\<^sub>p \<Union>\<^sub>p (map (\<lambda>xs. y ; Concat xs C) (a # ys))"
+      by (metis (no_types, lifting) Choice_prop_1_2 False choice_commute choice_commute_3 list.simps(9) map_is_Nil_conv)
+    then show ?thesis
+      by (smt (verit, best) \<open>Concat (y # a) C \<union>\<^sub>p \<Union>\<^sub>p (map ((\<lambda>xs. Concat xs C) \<circ> (#) y) ys) \<equiv>\<^sub>p Concat (y # a) C \<union>\<^sub>p \<Union>\<^sub>p (map (\<lambda>xs. y ; Concat xs C) ys)\<close> \<open>Concat (y # a) C \<union>\<^sub>p \<Union>\<^sub>p (map (\<lambda>xs. y ; Concat xs C) ys) \<equiv>\<^sub>p y ; Concat a C \<union>\<^sub>p \<Union>\<^sub>p (map (\<lambda>xs. y ; Concat xs C) ys)\<close> \<open>\<Union>\<^sub>p (Concat (y # a) C # map ((\<lambda>xs. Concat xs C) \<circ> (#) y) ys) = Concat (y # a) C \<union>\<^sub>p \<Union>\<^sub>p (map ((\<lambda>xs. Concat xs C) \<circ> (#) y) ys)\<close> \<open>\<Union>\<^sub>p (map ((\<lambda>xs. Concat xs C) \<circ> (#) y) (a # ys)) = \<Union>\<^sub>p (Concat (y # a) C # map ((\<lambda>xs. Concat xs C) \<circ> (#) y) ys)\<close> equiv_is_transitive)
+  qed
+qed
+
+theorem cnf2_prop9: "\<Union>\<^sub>p (map (\<lambda>xs. y ; Concat xs C) xs) \<equiv>\<^sub>p y ;  \<Union>\<^sub>p (map (\<lambda>xs. Concat xs C) xs)"
+proof (induction xs)
+  case Nil
+  then show ?case
+    apply auto
+    by (simp add: equiv_is_symetric fail_compose_r)
+next
+  case (Cons a xs)
+  have "\<Union>\<^sub>p (map (\<lambda>xs. y ; Concat xs C) (a # xs)) \<equiv>\<^sub>p y ; Concat a C \<union>\<^sub>p \<Union>\<^sub>p (map (\<lambda>xs. y ; Concat xs C) xs)"
+    by (metis (no_types, lifting) Choice.simps(2) Choice_prop_22 choice_commute choice_idem_2 choice_idem_3 equiv_is_symetric list.simps(9))
+  have "... \<equiv>\<^sub>p y ; Concat a C \<union>\<^sub>p y ; \<Union>\<^sub>p (map (\<lambda>xs. Concat xs C) xs)"
+    using choice_equiv equals_equiv_relation_3 local.Cons by blast
+  have "... \<equiv>\<^sub>p y ; (Concat a C \<union>\<^sub>p \<Union>\<^sub>p (map (\<lambda>xs. Concat xs C) xs))"
+    using compose_distrib1_3 equiv_is_symetric by blast
+  have "... \<equiv>\<^sub>p y ; \<Union>\<^sub>p (map (\<lambda>xs. Concat xs C) (a#xs))"
+    by (metis (no_types, lifting) Choice.simps(1) Choice.simps(2) Choice_prop_1_2 choice_commute composition_equiv equals_equiv_relation_3 fail_choice_l map_eq_Cons_conv)
+  then show ?case
+    using \<open>\<Union>\<^sub>p (map (\<lambda>xs. y ; Concat xs C) (a # xs)) \<equiv>\<^sub>p y ; Concat a C \<union>\<^sub>p \<Union>\<^sub>p (map (\<lambda>xs. y ; Concat xs C) xs)\<close> \<open>y ; Concat a C \<union>\<^sub>p \<Union>\<^sub>p (map (\<lambda>xs. y ; Concat xs C) xs) \<equiv>\<^sub>p y ; Concat a C \<union>\<^sub>p y ; \<Union>\<^sub>p (map (\<lambda>xs. Concat xs C) xs)\<close> \<open>y ; Concat a C \<union>\<^sub>p y ; \<Union>\<^sub>p (map (\<lambda>xs. Concat xs C) xs) \<equiv>\<^sub>p y ; (Concat a C \<union>\<^sub>p \<Union>\<^sub>p (map (\<lambda>xs. Concat xs C) xs))\<close> equiv_is_transitive by blast
+qed
+
+theorem cnf2_prop10: "is_feasible y \<Longrightarrow> S y \<subseteq> C \<Longrightarrow> y ; \<Union>\<^sub>p (map (\<lambda>xs. Concat xs C) ([x] \<interleave> ys)) \<equiv>\<^sub>p \<Union>\<^sub>p (map ((\<lambda>xs. Concat xs C) \<circ> (#) y) ([x] \<interleave> ys))"
+proof (induction ys)
+  case Nil
+  then show ?case apply auto
+    by (simp add: equals_equiv_relation_3)
+next
+  case (Cons a ys)
+  have "y ; \<Union>\<^sub>p (map (\<lambda>xs. Concat xs C) ([x] \<interleave> ys)) \<equiv>\<^sub>p \<Union>\<^sub>p (map ((\<lambda>xs. Concat xs C) \<circ> (#) y) ([x] \<interleave> ys))"
+    by (simp add: Cons.IH Cons.prems(1) Cons.prems(2))
+  have "y ; \<Union>\<^sub>p (map (\<lambda>xs. Concat xs C) ([x] \<interleave> (a # ys))) = y ; \<Union>\<^sub>p (foldl (;) (x ; a) ys # map ((\<lambda>xs. Concat xs C) \<circ> (#) a) ([x] \<interleave> ys))" by auto
+  have "\<Union>\<^sub>p (map ((\<lambda>xs. Concat xs C) \<circ> (#) y) ([x] \<interleave> (a # ys))) = \<Union>\<^sub>p (foldl (;) (y ; (x ; a)) ys # map ((\<lambda>xs. Concat xs C) \<circ> (#) y \<circ> (#) a) ([x] \<interleave> ys))" by auto
+  have "... = \<Union>\<^sub>p ((y ; foldl (;) ((x ; a)) ys) # map ((\<lambda>xs. Concat xs C) \<circ> (#) y \<circ> (#) a) ([x] \<interleave> ys))"
+    by (simp add: fold_compose)
+  have "... = \<Union>\<^sub>p ((y ; foldl (;) ((x ; a)) ys) # map ((\<lambda>xs. y ; Concat xs C) \<circ> (#) a) ([x] \<interleave> ys))"
+    by (smt (verit, best) Concat_prop_10 comp_apply list.discI map_eq_conv)
+  have "... = (y ; foldl (;) ((x ; a)) ys) \<union>\<^sub>p \<Union>\<^sub>p (map ((\<lambda>xs. y ; Concat xs C) \<circ> (#) a) ([x] \<interleave> ys))"
+    by (simp add: Choice_prop_1_2 inter_prop1)
+  have "... \<equiv>\<^sub>p (y ; foldl (;) ((x ; a)) ys) \<union>\<^sub>p y ; \<Union>\<^sub>p (map ((\<lambda>xs. Concat xs C) \<circ> (#) a) ([x] \<interleave> ys))"
+    using cnf2_prop9[of y C "map ((#) a) ([x] \<interleave> ys)"]
+    by (simp add: choice_equiv equals_equiv_relation_3)
+  have "... \<equiv>\<^sub>p y ; ((foldl (;) ((x ; a)) ys) \<union>\<^sub>p \<Union>\<^sub>p (map ((\<lambda>xs. Concat xs C) \<circ> (#) a) ([x] \<interleave> ys)))"
+    by (simp add: compose_distrib1_3 equiv_is_symetric)
+  have "... \<equiv>\<^sub>p y ; \<Union>\<^sub>p (map (\<lambda>xs. Concat xs C) ([x] \<interleave> (a # ys)))"
+    by (simp add: Choice_prop_1_2 equiv_is_reflexive inter_prop1)
+  then show "y ; \<Union>\<^sub>p (map (\<lambda>xs. Concat xs C) ([x] \<interleave> (a # ys))) \<equiv>\<^sub>p \<Union>\<^sub>p (map ((\<lambda>xs. Concat xs C) \<circ> (#) y) ([x] \<interleave> (a # ys)))"
+    by (smt (verit, best) \<open>\<Union>\<^sub>p (foldl (;) (y ; (x ; a)) ys # map ((\<lambda>xs. Concat xs C) \<circ> (#) y \<circ> (#) a) ([x] \<interleave> ys)) = \<Union>\<^sub>p (y ; foldl (;) (x ; a) ys # map ((\<lambda>xs. Concat xs C) \<circ> (#) y \<circ> (#) a) ([x] \<interleave> ys))\<close> \<open>\<Union>\<^sub>p (map ((\<lambda>xs. Concat xs C) \<circ> (#) y) ([x] \<interleave> (a # ys))) = \<Union>\<^sub>p (foldl (;) (y ; (x ; a)) ys # map ((\<lambda>xs. Concat xs C) \<circ> (#) y \<circ> (#) a) ([x] \<interleave> ys))\<close> \<open>\<Union>\<^sub>p (y ; foldl (;) (x ; a) ys # map ((\<lambda>xs. Concat xs C) \<circ> (#) y \<circ> (#) a) ([x] \<interleave> ys)) = \<Union>\<^sub>p (y ; foldl (;) (x ; a) ys # map ((\<lambda>xs. y ; Concat xs C) \<circ> (#) a) ([x] \<interleave> ys))\<close> \<open>\<Union>\<^sub>p (y ; foldl (;) (x ; a) ys # map ((\<lambda>xs. y ; Concat xs C) \<circ> (#) a) ([x] \<interleave> ys)) = y ; foldl (;) (x ; a) ys \<union>\<^sub>p \<Union>\<^sub>p (map ((\<lambda>xs. y ; Concat xs C) \<circ> (#) a) ([x] \<interleave> ys))\<close> \<open>y ; foldl (;) (x ; a) ys \<union>\<^sub>p \<Union>\<^sub>p (map ((\<lambda>xs. y ; Concat xs C) \<circ> (#) a) ([x] \<interleave> ys)) \<equiv>\<^sub>p y ; foldl (;) (x ; a) ys \<union>\<^sub>p y ; \<Union>\<^sub>p (map ((\<lambda>xs. Concat xs C) \<circ> (#) a) ([x] \<interleave> ys))\<close> \<open>y ; foldl (;) (x ; a) ys \<union>\<^sub>p y ; \<Union>\<^sub>p (map ((\<lambda>xs. Concat xs C) \<circ> (#) a) ([x] \<interleave> ys)) \<equiv>\<^sub>p y ; (foldl (;) (x ; a) ys \<union>\<^sub>p \<Union>\<^sub>p (map ((\<lambda>xs. Concat xs C) \<circ> (#) a) ([x] \<interleave> ys)))\<close> equiv_is_symetric equiv_is_transitive)
+qed
+
+theorem cnf2_prop11: "size xs = size ys \<Longrightarrow> \<forall>z \<in> set (zip xs ys). fst z \<equiv>\<^sub>p snd z \<Longrightarrow> \<Union>\<^sub>p xs \<equiv>\<^sub>p \<Union>\<^sub>p ys"
+proof (induction "zip xs ys" arbitrary: xs ys)
+  case Nil
+  then show ?case by (auto simp: fail_equiv)
+next
+  case (Cons z zip_xy)
+  obtain x xs' where "xs=x#xs'"
+    by (metis Cons.hyps(2) zip_eq_ConsE)
+  obtain y ys' where "ys=y#ys'"
+    by (metis Cons.hyps(2) zip_eq_ConsE)
+  have "zip xs' ys' = zip_xy"
+    using Cons.hyps(2) \<open>xs = x # xs'\<close> \<open>ys = y # ys'\<close> by auto
+  have "\<Union>\<^sub>p xs' \<equiv>\<^sub>p \<Union>\<^sub>p ys'"
+    using Cons.hyps(1) Cons.prems(1) Cons.prems(2) \<open>xs = x # xs'\<close> \<open>ys = y # ys'\<close> \<open>zip xs' ys' = zip_xy\<close> by force
+  have "x \<equiv>\<^sub>p y"
+    using Cons.prems(2) \<open>xs = x # xs'\<close> \<open>ys = y # ys'\<close> by force
+  have "\<Union>\<^sub>p (x#xs') \<equiv>\<^sub>p x \<union>\<^sub>p \<Union>\<^sub>p xs'"
+    by (metis Choice_prop_16 Choice_prop_22 choice_commute_3 choice_idem_2 equiv_is_transitive list.set_intros(1))
+  have "\<Union>\<^sub>p (y#ys') \<equiv>\<^sub>p y \<union>\<^sub>p \<Union>\<^sub>p ys'"
+    by (metis Choice_prop_16 Choice_prop_22 choice_commute_3 choice_idem_2 equiv_is_transitive list.set_intros(1))
+  have "x \<union>\<^sub>p \<Union>\<^sub>p xs' \<equiv>\<^sub>p y \<union>\<^sub>p \<Union>\<^sub>p ys'"
+    by (simp add: \<open>\<Union>\<^sub>p xs' \<equiv>\<^sub>p \<Union>\<^sub>p ys'\<close> \<open>x \<equiv>\<^sub>p y\<close> choice_equiv)
+  have "\<Union>\<^sub>p (x#xs') \<equiv>\<^sub>p \<Union>\<^sub>p (y#ys')"
+    by (meson \<open>\<Union>\<^sub>p (x # xs') \<equiv>\<^sub>p x \<union>\<^sub>p \<Union>\<^sub>p xs'\<close> \<open>\<Union>\<^sub>p (y # ys') \<equiv>\<^sub>p y \<union>\<^sub>p \<Union>\<^sub>p ys'\<close> \<open>x \<union>\<^sub>p \<Union>\<^sub>p xs' \<equiv>\<^sub>p y \<union>\<^sub>p \<Union>\<^sub>p ys'\<close> equiv_is_symetric equiv_is_transitive)
+  show "\<Union>\<^sub>p xs \<equiv>\<^sub>p \<Union>\<^sub>p ys"
+    by (simp add: \<open>\<Union>\<^sub>p (x # xs') \<equiv>\<^sub>p \<Union>\<^sub>p (y # ys')\<close> \<open>xs = x # xs'\<close> \<open>ys = y # ys'\<close>)
+qed 
+
+theorem cnf2_prop12: "is_feasible x \<Longrightarrow> S x \<subseteq> C \<Longrightarrow> evaluate (map ((#) x) xs) C \<equiv>\<^sub>p x ; evaluate xs C"
+proof -
+  assume "is_feasible x"
+  assume "S x \<subseteq> C"
+  have "\<forall> tr \<in> set xs. Concat (x#tr) C \<equiv>\<^sub>p x ; Concat tr C "
+    by (metis Big_choice.skip_prop Concat.simps(1) Concat.simps(2) Concat_prop_10 \<open>S x \<subseteq> C\<close> \<open>is_feasible x\<close> equiv_is_reflexive equiv_is_symetric)
+  have "\<forall>tr \<in> set (zip (map (\<lambda>tr. x ; Concat tr C) xs) (map (\<lambda>tr. Concat (x#tr) C) xs)). fst tr \<equiv>\<^sub>p snd tr "
+  proof auto
+    fix a b 
+    assume "(a, b) \<in> set (zip (map (\<lambda>tr. x ; Concat tr C) xs) (map (\<lambda>tr. Concat (x # tr) C) xs))"
+    have "zip (map (\<lambda>tr. x ; Concat tr C) xs) (map (\<lambda>tr. Concat (x # tr) C) xs) = (map (\<lambda>tr. (x ; Concat tr C, Concat (x # tr) C)) xs)" apply (induction xs) by auto
+    have "(a, b) \<in> set ((map (\<lambda>tr. (x ; Concat tr C, Concat (x # tr) C)) xs))"
+      using \<open>(a, b) \<in> set (zip (map (\<lambda>tr. x ; Concat tr C) xs) (map (\<lambda>tr. Concat (x # tr) C) xs))\<close> \<open>zip (map (\<lambda>tr. x ; Concat tr C) xs) (map (\<lambda>tr. Concat (x # tr) C) xs) = map (\<lambda>tr. (x ; Concat tr C, Concat (x # tr) C)) xs\<close> by force
+    then show "a \<equiv>\<^sub>p b" using \<open>\<forall> tr \<in> set xs. Concat (x#tr) C \<equiv>\<^sub>p x ; Concat tr C\<close> apply auto
+      using equiv_is_symetric by auto
+  qed
+  have "evaluate (map ((#) x) xs) C = \<Union>\<^sub>p (map ((\<lambda>tr. Concat tr C) \<circ> (#) x) xs)" by (auto simp: evaluate_def)
+  have "... = \<Union>\<^sub>p (map (\<lambda>tr. Concat (x#tr) C) xs)"
+    by (meson comp_apply)
+  have "... \<equiv>\<^sub>p \<Union>\<^sub>p (map (\<lambda>tr. x ; Concat tr C) xs)"
+    by (simp add: \<open>\<forall>tr\<in>set (zip (map (\<lambda>tr. x ; Concat tr C) xs) (map (\<lambda>tr. Concat (x # tr) C) xs)). fst tr \<equiv>\<^sub>p snd tr\<close> cnf2_prop11 equiv_is_symetric)
+  show "evaluate (map ((#) x) xs) C \<equiv>\<^sub>p x ; evaluate xs C"
+    by (metis (no_types, lifting) \<open>S x \<subseteq> C\<close> \<open>is_feasible x\<close> cnf2_prop8 cnf2_prop9 equiv_is_transitive evaluate_def map_map)
+qed
+
+
+theorem cnf_prop5: "all_feasible (xs@ys) \<Longrightarrow> complete_state (xs@ys) \<subseteq> C \<Longrightarrow> cnf_concurrency2 [xs] [ys] C \<equiv>\<^sub>p evaluate (xs \<interleave> ys) C"
+proof (induction xs arbitrary: ys)
+  case Nil
+  have "cnf_concurrency2 [[]] [ys] C = Concat ys C" by (auto simp: evaluate_def) 
+  then show ?case apply (auto simp: evaluate_def)
+    by (simp add: equiv_is_reflexive)
+next
+  case (Cons x xs)
+  then show ?case
+  proof (induction ys)
+    case Nil
+    then show ?case apply auto
+      by (simp add: equiv_is_reflexive)
+  next
+    case (Cons y ys)
+    have "cnf_concurrency2 [x # xs] [y # ys] C = x ; cnf_concurrency2 [xs] [y # ys] C \<union>\<^sub>p y ; cnf_concurrency2 [x # xs] [ys] C" by auto
+    have "evaluate (map ((#) x) (xs \<interleave> (y # ys))) C \<equiv>\<^sub>p x ; evaluate ((xs \<interleave> (y # ys))) C"
+      by (metis Cons.prems(2) Cons.prems(3) Cons_eq_appendI Un_subset_iff all_feasible.simps(2) cnf2_prop12 complete_state_prop)
+    have "evaluate (map ((#) y) ((x # xs) \<interleave> ys)) C \<equiv>\<^sub>p y ; evaluate ((x # xs) \<interleave> ys) C"
+      using Cons.prems(2) Cons.prems(3) Cons_eq_appendI Un_subset_iff all_feasible.simps(2) cnf2_prop12[of y C "(x # xs) \<interleave> ys"] complete_state_prop
+      by (metis complete_state_union_3 feas_prop2)
+    have "evaluate ((x # xs) \<interleave> (y # ys)) C = evaluate (map ((#) x) (xs \<interleave> (y # ys)) @ map ((#) y) ((x # xs) \<interleave> ys)) C" by auto
+
+    have "x ; evaluate ((xs \<interleave> (y # ys))) C \<equiv>\<^sub>p x ; cnf_concurrency2 [xs] [y # ys] C"
+      by (smt (verit, del_insts) Cons.prems(1) Cons.prems(2) Cons.prems(3) Un_subset_iff all_feasible.simps(2) cnf2_prop5 cnf2_prop7 complete_state_union_3 composition_equiv equiv_is_reflexive equiv_is_symetric feas_prop1 feas_prop2 feas_prop8 inter_prop1 interleave.simps(3) order.trans self_append_conv state_prop10)
+    have "y ; evaluate (((x # xs) \<interleave> ys)) C \<equiv>\<^sub>p y ; cnf_concurrency2 [x # xs] [ys] C"
+      using Cons.prems(1) Cons.prems(2) Cons.prems(3) Un_subset_iff all_feasible.simps(2) cnf2_prop5 cnf2_prop7 complete_state_union_3 composition_equiv equiv_is_reflexive equiv_is_symetric feas_prop1 feas_prop2 feas_prop8 inter_prop1 interleave.simps(3) order.trans self_append_conv state_prop10
+      by (smt (verit, ccfv_threshold) Cons.IH inverse_equality_2 le_supE list.distinct(1) state_prop11)
+    then show ?case
+      by (smt (verit) \<open>cnf_concurrency2 [x # xs] [y # ys] C = x ; cnf_concurrency2 [xs] [y # ys] C \<union>\<^sub>p y ; cnf_concurrency2 [x # xs] [ys] C\<close> \<open>evaluate ((x # xs) \<interleave> (y # ys)) C = evaluate (map ((#) x) (xs \<interleave> (y # ys)) @ map ((#) y) ((x # xs) \<interleave> ys)) C\<close> \<open>evaluate (map ((#) x) (xs \<interleave> (y # ys))) C \<equiv>\<^sub>p x ; evaluate (xs \<interleave> (y # ys)) C\<close> \<open>evaluate (map ((#) y) ((x # xs) \<interleave> ys)) C \<equiv>\<^sub>p y ; evaluate ((x # xs) \<interleave> ys) C\<close> \<open>x ; evaluate (xs \<interleave> (y # ys)) C \<equiv>\<^sub>p x ; cnf_concurrency2 [xs] [y # ys] C\<close> choice_equiv equiv_is_symetric equiv_is_transitive evaluate_split inter_size length_greater_0_conv list.map_disc_iff)
+  qed
+qed
+
+theorem cnf_prop3: "all_feasible (x#ys) \<Longrightarrow> complete_state (x#ys) \<subseteq> C \<Longrightarrow> cnf_concurrency2 [[x]] [ys] C \<equiv>\<^sub>p evaluate ([x] \<interleave> ys) C"
+proof (induction ys)
+  case Nil
+  then show ?case apply auto
+    by (simp add: equiv_is_reflexive)
+next
+  case (Cons a ys)
+  have "x ; Concat (a # ys) C = foldl (;) (x ; a) ys"
+    by (metis Concat_prop_1 foldl_Cons list.discI)
+  have "a ; \<Union>\<^sub>p (map (\<lambda>xs. Concat xs C) ([x] \<interleave> ys)) \<equiv>\<^sub>p \<Union>\<^sub>p (map ((\<lambda>xs. Concat xs C) \<circ> (#) a) ([x] \<interleave> ys))" using cnf2_prop9[of a C "[x] \<interleave> ys"] cnf2_prop8[of a C "[x] \<interleave> ys"]
+    by (smt (verit, ccfv_SIG) Cons.prems(1) Cons.prems(2) Un_subset_iff all_feasible.simps(2) complete_state_prop equiv_is_symetric equiv_is_transitive)
+  have "a ; evaluate ([x] \<interleave> ys) C \<union>\<^sub>p x ; evaluate [a # ys] C \<equiv>\<^sub>p evaluate ([x # a # ys]) C \<union>\<^sub>p evaluate (map ((#) a) ([x] \<interleave> ys)) C" apply (auto simp: evaluate_def)
+    using \<open>a ; \<Union>\<^sub>p (map (\<lambda>xs. Concat xs C) ([x] \<interleave> ys)) \<equiv>\<^sub>p \<Union>\<^sub>p (map ((\<lambda>xs. Concat xs C) \<circ> (#) a) ([x] \<interleave> ys))\<close> \<open>x ; Concat (a # ys) C = foldl (;) (x ; a) ys\<close> choice_equiv equals_equiv_relation_3 by blast
+  have "a ; evaluate ([x] \<interleave> ys) C \<union>\<^sub>p x ; evaluate [a # ys] C \<equiv>\<^sub>p evaluate ((x # a # ys) # map ((#) a) ([x] \<interleave> ys)) C"
+    by (simp add: \<open>a ; evaluate ([x] \<interleave> ys) C \<union>\<^sub>p x ; evaluate [a # ys] C \<equiv>\<^sub>p evaluate [x # a # ys] C \<union>\<^sub>p evaluate (map ((#) a) ([x] \<interleave> ys)) C\<close> concat_prop3 inter_prop1)
+  then show ?case
+    by (metis Cons.prems(1) Cons.prems(2) Cons_eq_appendI cnf_prop5 self_append_conv2)
+qed
+
+theorem cnf2_prop13: "all_feasible (x#xs@[y]) \<Longrightarrow> complete_state (x#xs@[y]) \<subseteq> C \<Longrightarrow> x ; cnf_concurrency2 [xs] [[y]] C \<equiv>\<^sub>p evaluate (map ((#) x) (xs \<interleave> [y])) C"
+proof (induction xs)
+  case Nil
+  then show ?case apply auto
+    by (simp add: cnf_prop equiv_is_reflexive)
+next
+  case (Cons a xs)
+  then have "all_feasible (xs)" and "is_feasible x" and "is_feasible a" and "is_feasible y" apply auto
+    using feas_prop1 apply blast
+    using all_feasible.simps(2) feas_prop2 by blast
+  moreover have "S x \<subseteq> C" and "S y \<subseteq> C" and "complete_state xs \<subseteq> C" and "S a \<subseteq> C"
+    using Cons.prems(2) complete_state_prop apply fastforce
+    apply (metis Cons.prems(2) complete_state_prop complete_state_union_3 dual_order.trans inf_sup_ord(4) le_supI1)
+    apply (metis Cons.prems(2) Un_subset_iff complete_state_union_1 complete_state_union_3) using Cons(3)
+    using fold_comp_prop3 state_composition_2 by fastforce
+  ultimately have "x ; cnf_concurrency2 [xs] [[y]] C \<equiv>\<^sub>p evaluate (map ((#) x) (xs \<interleave> [y])) C"
+    using Cons.IH Cons.prems(1) Cons.prems(2) all_feasible.simps(2) append_Cons complete_state_union_1 equalityE le_supI1 subset_trans
+    by (simp add: complete_state_prop)
+  have "evaluate (map ((#) x \<circ> (#) a) (xs \<interleave> [y]) @ [x # y # a # xs]) C \<equiv>\<^sub>p evaluate (map ((#) x \<circ> (#) a) (xs \<interleave> [y])) C \<union>\<^sub>p evaluate [x # y # a # xs] C"
+    using concat_prop5 by blast
+  have "x ; (y ; evaluate [a # xs] C \<union>\<^sub>p a ; cnf_concurrency2 [xs] [[y]] C) \<equiv>\<^sub>p x ; (y ; evaluate [a # xs] C) \<union>\<^sub>p x ; (a ; cnf_concurrency2 [xs] [[y]] C)"
+    using compose_distrib1_3 by auto
+  have "x ; (y ; evaluate [a # xs] C) = evaluate [x # y # a # xs] C"
+    by (simp add: cnf_prop)
+  have "cnf_feasible (xs \<interleave> [y])"
+    using Cons.prems(1) cnf2_prop4 by auto
+  then have "cnf_feasible (map ((#) a) (xs \<interleave> [y]))"
+    by (meson Cons.prems(1) all_feasible.simps(2) cnf2_prop2 feas_prop1)
+  then have "cnf_feasible ([x] # map ((#) a) (xs \<interleave> [y]))"
+    by (simp add: \<open>is_feasible x\<close>)
+  have "cnf_feasible ([x] # xs \<interleave> [y])"
+    using \<open>cnf_feasible ([x] # map ((#) a) (xs \<interleave> [y]))\<close> \<open>cnf_feasible (xs \<interleave> [y])\<close> cnf_feasible.simps(2) by blast
+  have "complete_cnf_state ((xs \<interleave> [y])) \<subseteq> C"
+    by (metis Cons.prems(2) Un_subset_iff cnf2_prop7 complete_state_prop complete_state_union_3)
+  then have "complete_cnf_state (map ((#) a) (xs \<interleave> [y])) \<subseteq> C"
+    by (metis \<open>S a \<subseteq> C\<close> cnf2_prop5 list.simps(8) sup.bounded_iff)
+  have "complete_cnf_state ([x] # xs \<interleave> [y]) \<subseteq> C" using \<open>complete_cnf_state ((xs \<interleave> [y])) \<subseteq> C\<close> \<open>S x \<subseteq> C\<close> apply (auto simp: complete_cnf_state_def)
+    by (simp add: Choice_state_1 in_mono)
+  have "cnf_feasible ([a] # xs \<interleave> [y])"
+    by (simp add: \<open>cnf_feasible (xs \<interleave> [y])\<close> \<open>is_feasible a\<close>)
+  have "complete_cnf_state ([a] # xs \<interleave> [y]) \<subseteq> C" using \<open>complete_cnf_state (xs \<interleave> [y]) \<subseteq> C\<close> \<open>S a \<subseteq> C\<close> apply (auto simp: complete_cnf_state_def)
+    by (simp add: Choice_state_1 in_mono)
+  have "all_feasible (xs @ [y])" and "complete_state (xs @ [y]) \<subseteq> C"
+    apply (simp add: \<open>all_feasible xs\<close> \<open>is_feasible y\<close> feas_prop8)
+    by (simp add: \<open>complete_cnf_state (xs \<interleave> [y]) \<subseteq> C\<close> cnf2_prop7 complete_state_union_3)
+
+
+  have "evaluate (map ((#) a) (xs \<interleave> [y])) C \<equiv>\<^sub>p a ; evaluate (xs \<interleave> [y]) C" using cnf2_prop12[of a C "(xs \<interleave> [y])"]
+    using \<open>cnf_feasible ([a] # xs \<interleave> [y])\<close> \<open>S a \<subseteq> C\<close> by auto
+  have "evaluate (map ((#) x \<circ> (#) a) (xs \<interleave> [y])) C \<equiv>\<^sub>p x ; evaluate (map ((#) a) (xs \<interleave> [y])) C" using cnf2_prop12[of x C "map ((#) a) (xs \<interleave> [y])"]
+    using \<open>cnf_feasible ([x] # map ((#) a) (xs \<interleave> [y]))\<close> \<open>S x \<subseteq> C\<close> by fastforce
+  have "... \<equiv>\<^sub>p x ; (a ; evaluate (xs \<interleave> [y]) C)"
+    by (simp add: \<open>evaluate (map ((#) a) (xs \<interleave> [y])) C \<equiv>\<^sub>p a ; evaluate (xs \<interleave> [y]) C\<close> composition_equiv equiv_is_reflexive)
+  have "x ; (a ; cnf_concurrency2 [xs] [[y]] C) \<equiv>\<^sub>p x ; evaluate (map ((#) a) (xs \<interleave> [y])) C"
+  proof-
+    have "x ; evaluate (map ((#) a) (xs \<interleave> [y])) C \<equiv>\<^sub>p x ; (a ; evaluate (xs \<interleave> [y]) C)"
+      by (simp add: \<open>x ; evaluate (map ((#) a) (xs \<interleave> [y])) C \<equiv>\<^sub>p x ; (a ; evaluate (xs \<interleave> [y]) C)\<close>)
+      have "... \<equiv>\<^sub>p x ; (a ; cnf_concurrency2 [xs] [[y]] C)" using cnf_prop5[of xs "[y]" C] \<open>all_feasible (xs @ [y])\<close> \<open>complete_state (xs @ [y]) \<subseteq> C\<close> apply auto
+        by (meson composition_equiv equiv_is_reflexive equiv_is_symetric)
+      show ?thesis
+        using \<open>x ; (a ; evaluate (xs \<interleave> [y]) C) \<equiv>\<^sub>p x ; (a ; cnf_concurrency2 [xs] [[y]] C)\<close> \<open>x ; evaluate (map ((#) a) (xs \<interleave> [y])) C \<equiv>\<^sub>p x ; (a ; evaluate (xs \<interleave> [y]) C)\<close> equiv_is_symetric equiv_is_transitive by blast
+    qed
+  then have "x ; (a ; cnf_concurrency2 [xs] [[y]] C) \<equiv>\<^sub>p evaluate (map ((#) x \<circ> (#) a) (xs \<interleave> [y])) C"
+    using \<open>evaluate (map ((#) x \<circ> (#) a) (xs \<interleave> [y])) C \<equiv>\<^sub>p x ; evaluate (map ((#) a) (xs \<interleave> [y])) C\<close> equiv_is_symetric equiv_is_transitive by blast
+  have "x ; (y ; evaluate [a # xs] C) \<union>\<^sub>p x ; (a ; cnf_concurrency2 [xs] [[y]] C) \<equiv>\<^sub>p evaluate (map ((#) x \<circ> (#) a) (xs \<interleave> [y])) C \<union>\<^sub>p evaluate [x # y # a # xs] C"
+    by (metis \<open>x ; (a ; cnf_concurrency2 [xs] [[y]] C) \<equiv>\<^sub>p evaluate (map ((#) x \<circ> (#) a) (xs \<interleave> [y])) C\<close> \<open>x ; (y ; evaluate [a # xs] C) = evaluate [x # y # a # xs] C\<close> choice_commute choice_equiv compose_assoc compose_assoc_3)
+  have "x ; (y ; evaluate [a # xs] C \<union>\<^sub>p a ; cnf_concurrency2 [xs] [[y]] C) \<equiv>\<^sub>p evaluate (map ((#) x \<circ> (#) a) (xs \<interleave> [y]) @ [x # y # a # xs]) C"
+    by (smt (verit) \<open>x ; (y ; evaluate [a # xs] C \<union>\<^sub>p a ; cnf_concurrency2 [xs] [[y]] C) \<equiv>\<^sub>p x ; (y ; evaluate [a # xs] C) \<union>\<^sub>p x ; (a ; cnf_concurrency2 [xs] [[y]] C)\<close> \<open>x ; (y ; evaluate [a # xs] C) \<union>\<^sub>p x ; (a ; cnf_concurrency2 [xs] [[y]] C) \<equiv>\<^sub>p evaluate (map ((#) x \<circ> (#) a) (xs \<interleave> [y])) C \<union>\<^sub>p evaluate [x # y # a # xs] C\<close> equiv_is_transitive eval_prop1 inter_prop1 interleave.elims list.discI map_is_Nil_conv)
+  then show ?case by simp
+qed
+
+theorem cnf2_prop14: "all_feasible (xs@ys) \<Longrightarrow> complete_state (xs@ys) \<subseteq> C \<Longrightarrow> cnf_concurrency2 [xs] [ys] C \<equiv>\<^sub>p evaluate ([xs] \<parallel> [ys]) C"
+proof (induction xs arbitrary: ys)
+  case Nil
+  then show ?case proof (induction ys)
+    case Nil
+    then show ?case by (auto simp: cnf_concurrency_def evaluate_def equiv_def) 
+  next
+    case (Cons y ys)
+    then show ?case
+      by (simp add: conc_prop2 equiv_def)
+  qed 
+next
+  case Con1: (Cons x xs)
+  have "all_feasible (xs @ ys)"
+    using Con1.prems(1) by auto
+  moreover have  "complete_state (xs @ ys) \<subseteq> C"
+    using Con1.prems(2) complete_state_union_1 by fastforce
+  moreover have "cnf_concurrency2 [xs] [ys] C \<equiv>\<^sub>p evaluate ([xs] \<parallel> [ys]) C"
+    by (simp add: Con1.IH \<open>all_feasible (xs @ ys)\<close> \<open>complete_state (xs @ ys) \<subseteq> C\<close>)
+  ultimately show ?case using Con1
+  proof (induction ys)
+    case Nil
+    then show ?case apply (induction xs)
+      by (auto simp add: conc_prop equiv_def)
+  next
+    case (Cons y ys)
+    have "all_feasible (xs @ ys)"
+      by (metis Cons.prems(1) all_feasible.simps(2) feas_prop1 feas_prop2 feas_prop8)
+    have "all_feasible ((x#xs) @ ys)"
+      using Con1.prems(1) \<open>all_feasible (xs @ ys)\<close> feas_prop1 feas_prop2 feas_prop8 by blast
+    have "all_feasible (xs @ (y#ys))"
+      by (simp add: Cons.prems(1))
+    have "all_feasible ((x#xs) @ (y#ys))"
+      using Cons.prems(5) by auto
+    have "is_feasible x"
+      using Con1.prems(1) by auto
+    have "is_feasible y"
+      using Cons.prems(1) all_feasible.simps(2) feas_prop2 by blast
+
+    have  "complete_state (xs @ ys) \<subseteq> C"
+      by (metis (full_types) Cons.prems(2) Un_subset_iff complete_state_prop complete_state_union_3)
+    have  "complete_state ((x#xs) @ ys) \<subseteq> C"
+      by (metis Cons.prems(6) Un_subset_iff \<open>complete_state (xs @ ys) \<subseteq> C\<close> complete_state_union_3)
+    have  "complete_state ((x#xs) @ (y#ys)) \<subseteq> C"
+      using Cons.prems(6) by blast
+    then have  "complete_state (x#xs) \<subseteq> C"
+      by (metis Un_subset_iff complete_state_union_3)
+    then have "S x \<subseteq> C" apply (auto simp: complete_state_def)
+      by (metis UnCI \<open>complete_state (x # xs) \<subseteq> C\<close> complete_state_prop sup.absorb_iff1)
+    then have  "complete_state (y#ys) \<subseteq> C"
+      by (metis Cons.prems(2) Un_subset_iff complete_state_union_3)
+    then have "S y \<subseteq> C" apply (auto simp: complete_state_def)
+      by (metis Cons.prems(6) UnCI complete_state_prop complete_state_union_3 subset_iff)
+    have "cnf_concurrency2 [xs] [ys] C \<equiv>\<^sub>p evaluate ([xs] \<parallel> [ys]) C"
+        by (simp add: Con1.IH \<open>all_feasible (xs @ ys)\<close> \<open>complete_state (xs @ ys) \<subseteq> C\<close>)
+    have "cnf_concurrency2 [x#xs] [ys] C \<equiv>\<^sub>p evaluate ([x#xs] \<parallel> [ys]) C"
+      using Con1.IH Cons.IH \<open>all_feasible ((x # xs) @ ys)\<close> \<open>all_feasible (xs @ ys)\<close> \<open>complete_state ((x # xs) @ ys) \<subseteq> C\<close> \<open>complete_state (xs @ ys) \<subseteq> C\<close> by blast
+    have "cnf_concurrency2 [xs] [y#ys] C \<equiv>\<^sub>p evaluate ([xs] \<parallel> [y#ys]) C"
+      by (simp add: Cons.prems(3))
+    have "cnf_feasible ([y] # [x] \<interleave> ys)"
+      by (metis Cons.prems(5) all_feasible.simps(1) all_feasible.simps(2) append_Cons cnf2_prop4 cnf_feasible.simps(2) feas_prop2 feas_prop8)
+    have "complete_cnf_state ([x] \<interleave> ys) = complete_state (x#ys)"
+      by (metis cnf2_prop7 complete_state_union_3 hd_step l8 tl_step)
+    then have "complete_cnf_state ([y] # [x] \<interleave> ys) = complete_cnf_state ([[y]]) \<union> complete_cnf_state ([x] \<interleave> ys)"
+      by (auto simp: complete_cnf_state_def)
+    have "... = S y \<union> complete_cnf_state ([x] \<interleave> ys)"
+      by (metis cnf2_prop7 complete_state_prop complete_state_union_1 interleave.simps(1) sup_commute)
+    have "... \<subseteq> C"
+      by (metis (no_types, lifting) Cons.prems(6) \<open>complete_cnf_state ([x] \<interleave> ys) = complete_state (x # ys)\<close> complete_state_prop complete_state_union_3 sup.boundedE sup_assoc sup_commute)
+    have "complete_cnf_state ([y] # [x] \<interleave> ys) \<subseteq> C"
+      using \<open>S y \<union> complete_cnf_state ([x] \<interleave> ys) \<subseteq> C\<close> \<open>complete_cnf_state ([y] # [x] \<interleave> ys) = complete_cnf_state [[y]] \<union> complete_cnf_state ([x] \<interleave> ys)\<close> \<open>complete_cnf_state [[y]] \<union> complete_cnf_state ([x] \<interleave> ys) = S y \<union> complete_cnf_state ([x] \<interleave> ys)\<close> by auto
+    show "cnf_concurrency2 [x # xs] [y # ys] C \<equiv>\<^sub>p evaluate ([x # xs] \<parallel> [y # ys]) C"
+    proof (cases "xs=[]")
+      case t1: True
+      then show ?thesis
+      proof (cases "ys=[]")
+        case True
+        have "evaluate ([[x]] \<parallel> [[y]]) C = x;y \<union>\<^sub>p y;x" by (auto simp: cnf_concurrency_def evaluate_def)
+        have "cnf_concurrency2 [[x]] [[y]] C = x;y \<union>\<^sub>p y;x"
+          using cnf_concurrency2_simp5 by blast
+        have "cnf_concurrency2 [[x]] [[y]] C = evaluate ([[x]] \<parallel> [[y]]) C"
+          using \<open>cnf_concurrency2 [[x]] [[y]] C = x ; y \<union>\<^sub>p y ; x\<close> \<open>evaluate ([[x]] \<parallel> [[y]]) C = x ; y \<union>\<^sub>p y ; x\<close> by presburger
+        then show ?thesis using t1
+          using True equiv_def by fastforce
+      next
+        case False
+        have "evaluate ([[x]] \<parallel> [y#ys]) C = evaluate ((x # y # ys) # map ((#) y) ([x] \<interleave> ys)) C" by (auto simp: cnf_concurrency_def)
+        have "cnf_concurrency2 [[x]] [y#ys] C = x ; evaluate [y # ys] C \<union>\<^sub>p y ; cnf_concurrency2 [[x]] [ys] C" by auto
+        have "cnf_concurrency2 [[x]] [ys] C \<equiv>\<^sub>p evaluate ([x] \<interleave> ys) C"
+          using \<open>all_feasible ((x # xs) @ ys)\<close> \<open>complete_state ((x # xs) @ ys) \<subseteq> C\<close> cnf_prop5 local.t1 by blast
+        have "evaluate (map ((#) y) ([x] \<interleave> ys)) C \<equiv>\<^sub>p y ; evaluate ([x] \<interleave> ys) C"
+          apply (simp add: evaluate_def) using cnf2_prop[of y "[x] \<interleave> ys" C]
+          using \<open>cnf_feasible ([y] # [x] \<interleave> ys)\<close> \<open>complete_cnf_state ([y] # [x] \<interleave> ys) \<subseteq> C\<close> by linarith
+        have "y ; evaluate ([x] \<interleave> ys) C  \<equiv>\<^sub>p evaluate (map ((#) y) ([x] \<interleave> ys)) C"
+          apply (simp add: evaluate_def) using cnf2_prop10[of y C x ys]
+          using Cons.prems(1) \<open>S y \<union> complete_cnf_state ([x] \<interleave> ys) \<subseteq> C\<close> local.t1 by fastforce
+        have "complete_state (y # x # ys) \<subseteq> C"
+          by (metis Un_commute \<open>complete_cnf_state ([x] \<interleave> ys) = complete_state (x # ys)\<close> \<open>complete_cnf_state ([y] # [x] \<interleave> ys) = complete_cnf_state [[y]] \<union> complete_cnf_state ([x] \<interleave> ys)\<close> \<open>complete_cnf_state ([y] # [x] \<interleave> ys) \<subseteq> C\<close> \<open>complete_cnf_state [[y]] \<union> complete_cnf_state ([x] \<interleave> ys) = S y \<union> complete_cnf_state ([x] \<interleave> ys)\<close> complete_state_prop)
+        have "all_feasible (y # x # ys)"
+          using \<open>all_feasible ((x # xs) @ ys)\<close> \<open>cnf_feasible ([y] # [x] \<interleave> ys)\<close> local.t1 by fastforce
+        have "y ; cnf_concurrency2 [[x]] [ys] C  \<equiv>\<^sub>p evaluate (map ((#) y) ([x] \<interleave> ys)) C"
+          apply (auto simp: evaluate_def)
+        proof -
+          have "\<Union>\<^sub>p (map ((\<lambda>xs. Concat xs C) \<circ> (#) y) ([x] \<interleave> ys)) \<equiv>\<^sub>p y ; \<Union>\<^sub>p (map ((\<lambda>xs. Concat xs C)) ([x] \<interleave> ys))"
+            using cnf2_prop10[of y C x ys] equiv_is_symetric \<open>S y \<subseteq> C\<close> \<open>all_feasible (y # x # ys)\<close> by auto
+          have "... \<equiv>\<^sub>p y ; cnf_concurrency2 [[x]] [ys] C"
+            using cnf_prop5[of "[x]" ys C] equiv_is_reflexive evaluate_def
+            by (metis \<open>cnf_concurrency2 [[x]] [ys] C \<equiv>\<^sub>p evaluate ([x] \<interleave> ys) C\<close> composition_equiv equiv_is_symetric)
+          show "y ; cnf_concurrency2 [[x]] [ys] C \<equiv>\<^sub>p \<Union>\<^sub>p (map ((\<lambda>xs. Concat xs C) \<circ> (#) y) ([x] \<interleave> ys))"
+            using \<open>\<Union>\<^sub>p (map ((\<lambda>xs. Concat xs C) \<circ> (#) y) ([x] \<interleave> ys)) \<equiv>\<^sub>p y ; \<Union>\<^sub>p (map (\<lambda>xs. Concat xs C) ([x] \<interleave> ys))\<close> \<open>y ; \<Union>\<^sub>p (map (\<lambda>xs. Concat xs C) ([x] \<interleave> ys)) \<equiv>\<^sub>p y ; cnf_concurrency2 [[x]] [ys] C\<close> equiv_is_symetric equiv_is_transitive by blast
+        qed
+        have "x ; evaluate [y # ys] C \<union>\<^sub>p y ; cnf_concurrency2 [[x]] [ys] C  \<equiv>\<^sub>p evaluate ((x # y # ys) # map ((#) y) ([x] \<interleave> ys)) C"
+          by (metis False \<open>y ; cnf_concurrency2 [[x]] [ys] C \<equiv>\<^sub>p evaluate (map ((#) y) ([x] \<interleave> ys)) C\<close> choice_equiv cnf_prop compose_assoc compose_assoc_3 concat_prop3 inter_prop1 list.discI list.map_disc_iff)
+           
+        have "cnf_concurrency2 [[x]] [y#ys] C  \<equiv>\<^sub>p evaluate ([[x]] \<parallel> [y#ys] ) C"
+          by (simp add: \<open>evaluate ([[x]] \<parallel> [y # ys]) C = evaluate ((x # y # ys) # map ((#) y) ([x] \<interleave> ys)) C\<close> \<open>x ; evaluate [y # ys] C \<union>\<^sub>p y ; cnf_concurrency2 [[x]] [ys] C \<equiv>\<^sub>p evaluate ((x # y # ys) # map ((#) y) ([x] \<interleave> ys)) C\<close>)
+        then show ?thesis using t1
+          by blast
+      qed
+    next
+      case f1: False
+      then show ?thesis
+      proof (cases "ys=[]")
+        case True
+        have "evaluate ([x # xs] \<parallel> [[y]]) C = evaluate (map ((#) x) (xs \<interleave> [y]) @ [y # x # xs]) C" by (auto simp: cnf_concurrency_def)
+        have "... = evaluate ((y # x # xs) # (map ((#) x) (xs \<interleave> [y]))) C"
+          by (simp add: evaluate_switch)
+        have "... = y ; evaluate [x # xs] C \<union>\<^sub>p evaluate (map ((#) x) (xs \<interleave> [y])) C"
+          by (metis Cons_eq_appendI append_is_Nil_conv cnf_prop evaluate_split f1 inter_prop1 list.map_disc_iff not_Cons_self2 self_append_conv2)
+        have "all_feasible (x#xs@[y])"
+          using Cons.prems(5) True by auto
+        have "complete_state (x#xs@[y]) \<subseteq> C"
+          using Cons.prems(6) True by auto
+        have "evaluate (map ((#) x) (xs \<interleave> [y])) C \<equiv>\<^sub>p x ; evaluate (xs \<interleave> [y]) C"
+          using \<open>all_feasible (x # xs @ [y])\<close> \<open>complete_state (x # xs @ [y]) \<subseteq> C\<close> cnf2_prop13 cnf_prop5 equiv_is_symetric
+          by (simp add: \<open>S x \<subseteq> C\<close> cnf2_prop12)
+        have "x ; cnf_concurrency2 [xs] [[y]] C \<equiv>\<^sub>p evaluate (map ((#) x) (xs \<interleave> [y])) C"
+          using \<open>all_feasible (x # xs @ [y])\<close> \<open>complete_state (x # xs @ [y]) \<subseteq> C\<close> cnf2_prop13 by blast
+        then have "y ; evaluate [x # xs] C \<union>\<^sub>p x ; cnf_concurrency2 [xs] [[y]] C \<equiv>\<^sub>p y ; evaluate [x # xs] C \<union>\<^sub>p evaluate (map ((#) x) (xs \<interleave> [y])) C"
+          by (simp add: choice_equiv equiv_is_reflexive)
+        have "y ; evaluate [x # xs] C \<union>\<^sub>p x ; cnf_concurrency2 [xs] [[y]] C \<equiv>\<^sub>p evaluate ([x # xs] \<parallel> [[y]]) C"
+          by (simp add: \<open>evaluate ((y # x # xs) # map ((#) x) (xs \<interleave> [y])) C = y ; evaluate [x # xs] C \<union>\<^sub>p evaluate (map ((#) x) (xs \<interleave> [y])) C\<close> \<open>evaluate ([x # xs] \<parallel> [[y]]) C = evaluate (map ((#) x) (xs \<interleave> [y]) @ [y # x # xs]) C\<close> \<open>evaluate (map ((#) x) (xs \<interleave> [y]) @ [y # x # xs]) C = evaluate ((y # x # xs) # map ((#) x) (xs \<interleave> [y])) C\<close> \<open>y ; evaluate [x # xs] C \<union>\<^sub>p x ; cnf_concurrency2 [xs] [[y]] C \<equiv>\<^sub>p y ; evaluate [x # xs] C \<union>\<^sub>p evaluate (map ((#) x) (xs \<interleave> [y])) C\<close>)
+        then show ?thesis
+          using True by auto
+      next
+        case False
+        have "cnf_feasible ([x] # xs \<interleave> (y # ys))"
+          using Cons.prems(5) cnf2_prop4 by auto
+        have "cnf_feasible ([y] # (x # xs) \<interleave> ys)"
+          using \<open>all_feasible ((x # xs) @ ys)\<close> \<open>cnf_feasible ([y] # [x] \<interleave> ys)\<close> cnf2_prop4 cnf_feasible.simps(2) by blast
+        
+        have "complete_cnf_state ([x] # xs \<interleave> (y # ys)) \<subseteq> C"
+          by (metis (no_types, opaque_lifting) Cons.prems(2) Cons_eq_appendI \<open>S y \<union> complete_cnf_state ([x] \<interleave> ys) \<subseteq> C\<close> cnf2_prop6 cnf2_prop7 complete_state_union_3 interleave.simps(2) self_append_conv2 sup.bounded_iff)
+        have "complete_cnf_state ([y] # (x # xs) \<interleave> ys) \<subseteq> C"
+          by (metis Cons_eq_appendI \<open>complete_cnf_state ([x] # xs \<interleave> (y # ys)) \<subseteq> C\<close> cnf2_prop6 cnf2_prop7 complete_state_union_1 complete_state_union_3 interleave.simps(1) self_append_conv2)
+        have "evaluate (map ((#) x) (xs \<interleave> (y # ys)) @ map ((#) y) ((x # xs) \<interleave> ys)) C = evaluate (map ((#) x) (xs \<interleave> (y # ys))) C \<union>\<^sub>p evaluate (map ((#) y) ((x # xs) \<interleave> ys)) C"
+          by (simp add: evaluate_split f1 inter_prop1)
+        have "evaluate (map ((#) x) (xs \<interleave> (y # ys))) C \<equiv>\<^sub>p x ; evaluate ((xs \<interleave> (y # ys))) C" using cnf2_prop12[of x C "xs \<interleave> (y # ys)"]
+          using Con1.prems(1) \<open>S x \<subseteq> C\<close> by auto
+        have "evaluate (map ((#) y) ((x # xs) \<interleave> ys)) C \<equiv>\<^sub>p y ; evaluate (((x # xs) \<interleave> ys)) C"
+          using \<open>is_feasible x\<close> \<open>S x \<subseteq> C\<close> cnf2_prop12
+          using \<open>S y \<subseteq> C\<close> \<open>is_feasible y\<close> by auto
+
+        have "x ; cnf_concurrency2 [xs] [y # ys] C \<union>\<^sub>p y ; cnf_concurrency2 [x # xs] [ys] C \<equiv>\<^sub>p evaluate (map ((#) x) (xs \<interleave> (y # ys)) @ map ((#) y) ((x # xs) \<interleave> ys)) C"
+          using cnf_concurrency2_simp8 cnf_prop5 interleave.simps(3)
+          by (metis Cons.prems(5) Cons.prems(6))
+        then show ?thesis by (auto simp: cnf_concurrency_def)
+      qed
+    qed
+  qed
+qed
+
+theorem cnf2_prop15: "cnf_feasible (x#ys) \<Longrightarrow> complete_cnf_state (x#ys) \<subseteq> C \<Longrightarrow> cnf_concurrency2 [x] ys C \<equiv>\<^sub>p evaluate(concat (map ((\<interleave>) x) ys)) C"
+proof (induction ys)
+  case Nil
+  then show ?case
+    apply (auto simp: evaluate_def)
+    by (simp add: fail_equiv)
+next
+  case (Cons y ys)
+  have "cnf_concurrency2 [x] (y # ys) C \<equiv>\<^sub>p cnf_concurrency2 [x] [y] C \<union>\<^sub>p cnf_concurrency2 [x] ys C"
+    by (metis choice_commute choice_commute_3 cnf_concurrency2_simp12 cnf_concurrency2_simp2 equiv_is_symetric fail_choice_l permutations.elims)
+  have "evaluate (x \<interleave> y @ concat (map ((\<interleave>) x) ys)) C \<equiv>\<^sub>p evaluate (x \<interleave> y) C \<union>\<^sub>p evaluate (concat (map ((\<interleave>) x) ys)) C"
+    using concat_prop5 by auto
+  have "all_feasible (x @ y)" and "complete_state (x @ y) \<subseteq> C"
+    using Cons.prems(1) feas_prop8 apply auto[1] using Cons.prems(2) apply (auto simp: complete_cnf_state_def)
+  proof -
+    fix xa :: 'a
+    assume a1: "xa \<in> complete_state (x @ y)"
+    have "\<forall>ps pss pssa pssb. ((ps::'a Program list) # pss = pssa @ pssb \<or> (\<forall>pssc. pssc @ pssb \<noteq> pss \<or> ps # pssc \<noteq> pssa) \<and> (ps # pss \<noteq> pssb \<or> [] \<noteq> pssa)) \<and> ((\<exists>pssc. pssc @ pssb = pss \<and> ps # pssc = pssa) \<or> ps # pss = pssb \<and> [] = pssa \<or> ps # pss \<noteq> pssa @ pssb)"
+      by (metis (no_types) Cons_eq_append_conv)
+    then obtain ppss :: "'a Program list \<Rightarrow> 'a Program list list \<Rightarrow> 'a Program list list \<Rightarrow> 'a Program list list \<Rightarrow> 'a Program list list" and ppssa :: "'a Program list \<Rightarrow> 'a Program list list \<Rightarrow> 'a Program list list \<Rightarrow> 'a Program list list \<Rightarrow> 'a Program list list" where
+      f2: "\<forall>ps pss pssa pssb. (ps # pss = pssa @ pssb \<or> (\<forall>pssc. pssc @ pssb \<noteq> pss \<or> ps # pssc \<noteq> pssa) \<and> (ps # pss \<noteq> pssb \<or> [] \<noteq> pssa)) \<and> (ppss ps pss pssa pssb @ pssb = pss \<and> ps # ppss ps pss pssa pssb = pssa \<or> ps # pss = pssb \<and> [] = pssa \<or> ps # pss \<noteq> pssa @ pssb)"
+      by moura
+    have "\<forall>pss. ([]::'a Program list list) @ pss = pss"
+      by fastforce
+    then show "xa \<in> C"
+      using f2 a1 by (metis (no_types) Cons.prems(2) state_prop10 state_prop9 subset_iff)
+  qed
+  have "cnf_concurrency2 [x] [y] C \<equiv>\<^sub>p evaluate (x \<interleave> y) C"
+    using cnf_prop5[of x y C] equals_equiv_relation_3
+    using \<open>all_feasible (x @ y)\<close> \<open>complete_state (x @ y) \<subseteq> C\<close> by blast
+  have "cnf_concurrency2 [x] ys C \<equiv>\<^sub>p evaluate (concat (map ((\<interleave>) x) ys)) C"
+    by (metis (no_types, lifting) Cons.IH Cons.prems(1) Cons.prems(2) cnf_choice2 cnf_feasible.simps(2) dual_order.trans state_prop12 subset3)
+  have "cnf_concurrency2 [x] (y # ys) C \<equiv>\<^sub>p evaluate (x \<interleave> y @ concat (map ((\<interleave>) x) ys)) C"
+    by (meson \<open>cnf_concurrency2 [x] (y # ys) C \<equiv>\<^sub>p cnf_concurrency2 [x] [y] C \<union>\<^sub>p cnf_concurrency2 [x] ys C\<close> \<open>cnf_concurrency2 [x] [y] C \<equiv>\<^sub>p evaluate (x \<interleave> y) C\<close> \<open>cnf_concurrency2 [x] ys C \<equiv>\<^sub>p evaluate (concat (map ((\<interleave>) x) ys)) C\<close> choice_equiv concat_prop5 equiv_is_symetric equiv_is_transitive)
+  then show ?case by auto
+qed
+
+theorem cnf2_prop16: "cnf_feasible (xs @ ys) \<Longrightarrow> cnf_feasible ys"
+  apply (induction xs) by auto
+theorem cnf2_prop17: "cnf_feasible (xs @ ys) \<Longrightarrow> cnf_feasible xs"
+  apply (induction xs) by auto
+
+theorem "cnf_feasible (xs @ ys) \<Longrightarrow> complete_cnf_state (xs @ ys) \<subseteq> C \<Longrightarrow> cnf_concurrency2 xs ys C \<equiv>\<^sub>p evaluate (xs \<parallel> ys) C"
+proof (induction xs)
+  case Nil
+  then show ?case 
+    apply (auto simp: evaluate_def cnf_concurrency_def)
+    by (simp add: fail_equiv)
+next
+  case Cons1: (Cons x xs)
+  then show ?case
+  proof (induction ys)
+    case Nil
+    then show ?case apply (auto simp: evaluate_def cnf_concurrency_def)
+      by (meson cnf_state_prop)
+  next
+    case (Cons y ys)
+    have "cnf_feasible (y#ys)" using Cons(3)
+      using cnf2_prop16 by blast
+    then have "all_feasible (x @ y)" using  Cons(3) apply (auto simp: complete_cnf_state_def cnf_feasible_def)
+      by (simp add: feas_prop8)
+    have "complete_cnf_state (x # xs) \<subseteq> C"
+      by (meson Cons.prems(3) state_prop10 subset_trans)
+    then have "complete_state x \<subseteq> C" by (auto simp: complete_cnf_state_def)
+    have "complete_cnf_state (y # ys) \<subseteq> C"
+      by (meson Cons.prems(3) dual_order.trans state_prop11)
+    then have "complete_state y \<subseteq> C" by (auto simp: complete_cnf_state_def)
+    have "complete_state (x @ y) \<subseteq> C"
+      by (simp add: \<open>complete_state x \<subseteq> C\<close> \<open>complete_state y \<subseteq> C\<close> complete_state_union_3)
+    from Cons show "cnf_concurrency2 (x # xs) (y # ys) C \<equiv>\<^sub>p evaluate ((x # xs) \<parallel> (y # ys)) C"
+    proof (cases "xs=[]")
+      case t1: True
+      then show ?thesis
+      proof (cases "ys=[]")
+        case True
+        then show ?thesis using t1 apply simp using cnf2_prop14[of x y C]
+          using Cons.prems(2) Cons.prems(3) feas_prop8 state_prop9 by fastforce
+      next
+        case False
+        have "cnf_concurrency2 [x] (y # ys) C = cnf_concurrency2 [x] [y] C \<union>\<^sub>p cnf_concurrency2 [x] ys C"
+          by (metis False cnf_concurrency2_simp12 cnf_size.cases)
+        have "evaluate (x \<interleave> y @ concat (map ((\<interleave>) x) ys)) C \<equiv>\<^sub>p evaluate (x \<interleave> y) C \<union>\<^sub>p evaluate(concat (map ((\<interleave>) x) ys)) C" using False
+          by (simp add: concat_prop5)
+        have "cnf_concurrency2 [x] [y] C \<equiv>\<^sub>p evaluate (x \<interleave> y) C" using cnf_prop5[of x y C]
+          by (simp add: \<open>all_feasible (x @ y)\<close> \<open>complete_state (x @ y) \<subseteq> C\<close>)
+        have "cnf_concurrency2 [x] ys C \<equiv>\<^sub>p evaluate(concat (map ((\<interleave>) x) ys)) C" using cnf2_prop15
+          by (metis Cons1.prems(1) \<open>cnf_feasible (y # ys)\<close> \<open>complete_cnf_state (x # xs) \<subseteq> C\<close> \<open>complete_cnf_state (y # ys) \<subseteq> C\<close> append_Cons cnf2_prop6 cnf_feasible.simps(2) eq_Nil_appendI le_sup_iff)
+        have "cnf_concurrency2 [x] [y] C \<union>\<^sub>p cnf_concurrency2 [x] ys C \<equiv>\<^sub>p evaluate (x \<interleave> y) C \<union>\<^sub>p evaluate(concat (map ((\<interleave>) x) ys)) C"
+          using \<open>cnf_concurrency2 [x] ys C \<equiv>\<^sub>p evaluate (concat (map ((\<interleave>) x) ys)) C\<close> choice_equiv cnf_prop5 equiv_is_reflexive
+          using \<open>cnf_concurrency2 [x] [y] C \<equiv>\<^sub>p evaluate (x \<interleave> y) C\<close> by blast
+        have "cnf_concurrency2 [x] (y # ys) C \<equiv>\<^sub>p evaluate (x \<interleave> y @ concat (map ((\<interleave>) x) ys)) C"
+          using \<open>cnf_concurrency2 [x] (y # ys) C = cnf_concurrency2 [x] [y] C \<union>\<^sub>p cnf_concurrency2 [x] ys C\<close> \<open>cnf_concurrency2 [x] [y] C \<union>\<^sub>p cnf_concurrency2 [x] ys C \<equiv>\<^sub>p evaluate (x \<interleave> y) C \<union>\<^sub>p evaluate (concat (map ((\<interleave>) x) ys)) C\<close> \<open>evaluate (x \<interleave> y @ concat (map ((\<interleave>) x) ys)) C \<equiv>\<^sub>p evaluate (x \<interleave> y) C \<union>\<^sub>p evaluate (concat (map ((\<interleave>) x) ys)) C\<close> equiv_is_symetric equiv_is_transitive by fastforce
+        then show ?thesis using t1 by (auto simp: cnf_concurrency_def)
+      qed
+    next
+      case f1: False
+      then show ?thesis 
+      proof (cases "ys=[]")
+        case True
+        have "cnf_concurrency2 (x # xs) [y] C = cnf_concurrency2 [x] [y] C \<union>\<^sub>p cnf_concurrency2 xs [y] C"
+          by (metis cnf_concurrency2_simp11 cnf_size.cases f1)
+        have "concat (map (\<lambda>path_m. path_m \<interleave> y) xs) = xs \<parallel> [y]" by (auto simp: cnf_concurrency_def)
+        have "evaluate (x \<interleave> y @ concat (map (\<lambda>path_m. path_m \<interleave> y) xs)) C \<equiv>\<^sub>p evaluate (x \<interleave> y) C \<union>\<^sub>p evaluate (xs \<parallel> [y]) C"
+          by (simp add: \<open>concat (map (\<lambda>path_m. path_m \<interleave> y) xs) = xs \<parallel> [y]\<close> concat_prop5)
+        have "cnf_concurrency2 [x] [y] C \<equiv>\<^sub>p evaluate (x \<interleave> y) C"
+          using cnf_prop5[of x y C] equals_equiv_relation_3
+          using \<open>all_feasible (x @ y)\<close> \<open>complete_state (x @ y) \<subseteq> C\<close> by blast
+        have "cnf_concurrency2 xs [y] C \<equiv>\<^sub>p evaluate (xs \<parallel> [y]) C"
+          by (metis Cons.prems(1) Cons.prems(2) Cons.prems(3) True append_Cons cnf_feasible.simps(2) cnf_state_prop)
+        have "cnf_concurrency2 (x # xs) [y] C \<equiv>\<^sub>p evaluate ((x \<interleave> y) @ (xs \<parallel> [y])) C"
+          by (smt (verit) \<open>cnf_concurrency2 (x # xs) [y] C = cnf_concurrency2 [x] [y] C \<union>\<^sub>p cnf_concurrency2 xs [y] C\<close> \<open>cnf_concurrency2 [x] [y] C \<equiv>\<^sub>p evaluate (x \<interleave> y) C\<close> \<open>cnf_concurrency2 xs [y] C \<equiv>\<^sub>p evaluate (xs \<parallel> [y]) C\<close> choice_equiv concat_prop5 equiv_is_symetric equiv_is_transitive)
+        then show ?thesis using True by (auto simp: cnf_concurrency_def)
+      next
+        case False
+        obtain xx xs' where "xs=xx#xs'"
+          using cnf_size.cases f1 by blast
+        obtain yy ys' where "ys=yy#ys'"
+          using False cnf_size.cases by auto
+        have "cnf_concurrency2 (x # xs) (y # ys) C = cnf_concurrency2 (x # xx # xs') (y # yy # ys') C"
+          by (simp add: \<open>xs = xx # xs'\<close> \<open>ys = yy # ys'\<close>)
+        have "... = cnf_concurrency2 [x] (y # yy # ys') C \<union>\<^sub>p cnf_concurrency2 (xx # xs') (y # yy # ys') C"
+          using cnf_concurrenc2_simp16[of x xx xs' y yy ys' C] by simp
+        have "... = cnf_concurrency2 [x] (y # ys) C \<union>\<^sub>p cnf_concurrency2 xs (y # ys) C"
+          by (simp add: \<open>xs = xx # xs'\<close> \<open>ys = yy # ys'\<close>)
+        have "... = (cnf_concurrency2 [x] [y] C \<union>\<^sub>p cnf_concurrency2 [x] ys C) \<union>\<^sub>p cnf_concurrency2 xs (y # ys) C"
+          by (simp add: \<open>ys = yy # ys'\<close>)
+        have "(x # xs) \<parallel> (y # ys) = (x \<interleave> y @ concat (map ((\<interleave>) x) ys) @ (xs \<parallel> (y#ys)))"
+          by (auto simp: cnf_concurrency_def)
+
+        have "evaluate ((x # xs) \<parallel> (y # ys)) C = evaluate (x \<interleave> y @ concat (map ((\<interleave>) x) (yy#ys')) @ ((xx#xs') \<parallel> (y#yy#ys'))) C" using \<open>xs=xx#xs'\<close> \<open>ys=yy#ys'\<close> by (auto simp: cnf_concurrency_def)
+        have "... = evaluate (x \<interleave> y) C \<union>\<^sub>p evaluate (concat (map ((\<interleave>) x) (yy#ys')) @ ((xx#xs') \<parallel> (y#yy#ys'))) C"
+          by (metis (no_types, opaque_lifting) List.bind_def append_is_Nil_conv bind_simps(2) evaluate_split inter_prop1 interleave.simps(1) neq_Nil_conv)
+        have "concat (map ((\<interleave>) x) (yy # ys')) \<noteq> []" and "(xx # xs') \<parallel> (y # yy # ys') \<noteq> []" apply auto
+          apply (metis interleav_lower_bound list.size(3) not_one_le_zero) apply (auto simp: cnf_concurrency_def)
+          using inter_size by blast
+        then have "evaluate (concat (map ((\<interleave>) x) (yy#ys')) @ ((xx#xs') \<parallel> (y#yy#ys'))) C = evaluate (concat (map ((\<interleave>) x) (yy#ys'))) C \<union>\<^sub>p evaluate ((xx#xs') \<parallel> (y#yy#ys')) C"
+          using evaluate_split[of "concat (map ((\<interleave>) x) (yy#ys'))" "(xx#xs') \<parallel> (y#yy#ys')" C] by auto
+        have "evaluate (x \<interleave> y @ concat (map ((\<interleave>) x) (yy#ys')) @ ((xx#xs') \<parallel> (y#yy#ys'))) C = evaluate (x \<interleave> y) C \<union>\<^sub>p (evaluate (concat (map ((\<interleave>) x) (yy#ys'))) C \<union>\<^sub>p evaluate ((xx#xs') \<parallel> (y#yy#ys')) C)"
+          using \<open>evaluate (concat (map ((\<interleave>) x) (yy # ys')) @ (xx # xs') \<parallel> (y # yy # ys')) C = evaluate (concat (map ((\<interleave>) x) (yy # ys'))) C \<union>\<^sub>p evaluate ((xx # xs') \<parallel> (y # yy # ys')) C\<close> \<open>evaluate (x \<interleave> y @ concat (map ((\<interleave>) x) (yy # ys')) @ (xx # xs') \<parallel> (y # yy # ys')) C = evaluate (x \<interleave> y) C \<union>\<^sub>p evaluate (concat (map ((\<interleave>) x) (yy # ys')) @ (xx # xs') \<parallel> (y # yy # ys')) C\<close> by auto
+        have "evaluate (x \<interleave> y @ concat (map ((\<interleave>) x) ys) @ (xs \<parallel> (y#ys))) C = evaluate (x \<interleave> y) C \<union>\<^sub>p (evaluate (concat (map ((\<interleave>) x) ys)) C \<union>\<^sub>p evaluate (xs \<parallel> (y#ys)) C)"
+          using \<open>evaluate (x \<interleave> y @ concat (map ((\<interleave>) x) (yy # ys')) @ (xx # xs') \<parallel> (y # yy # ys')) C = evaluate (x \<interleave> y) C \<union>\<^sub>p (evaluate (concat (map ((\<interleave>) x) (yy # ys'))) C \<union>\<^sub>p evaluate ((xx # xs') \<parallel> (y # yy # ys')) C)\<close> \<open>xs = xx # xs'\<close> \<open>ys = yy # ys'\<close> by blast
+
+        have "cnf_feasible (x # ys)"
+          using \<open>all_feasible (x @ y)\<close> \<open>cnf_feasible (y # ys)\<close> feas_prop1 by auto
+        have "complete_cnf_state ys \<subseteq> C" using \<open>complete_cnf_state (y#ys) \<subseteq> C\<close>
+          using cnf_state_prop by blast
+        have "complete_cnf_state (x # ys) \<subseteq> C" using \<open>complete_state x \<subseteq> C\<close> \<open>complete_cnf_state ys \<subseteq> C\<close> by (auto simp: complete_cnf_state_def)
+
+        have "evaluate (x \<interleave> y) C \<equiv>\<^sub>p cnf_concurrency2 [x] [y] C" using cnf_prop5
+          by (metis \<open>all_feasible (x @ y)\<close> \<open>complete_state (x @ y) \<subseteq> C\<close> equiv_is_symetric)
+        have "cnf_concurrency2 [x] ys C \<equiv>\<^sub>p evaluate (concat (map ((\<interleave>) x) ys)) C" using cnf2_prop15[of x ys C]
+          using \<open>cnf_feasible (x # ys)\<close> \<open>complete_cnf_state (x # ys) \<subseteq> C\<close> by auto
+        have "cnf_concurrency2 xs (y # ys) C \<equiv>\<^sub>p evaluate (xs \<parallel> (y#ys)) C"
+          using Cons.prems(1) Cons.prems(2) Cons.prems(3) cnf_state_prop by fastforce
+
+        have "evaluate (x \<interleave> y) C \<union>\<^sub>p         (evaluate (concat (map ((\<interleave>) x) ys)) C \<union>\<^sub>p evaluate (xs \<parallel> (y#ys)) C) \<equiv>\<^sub>p 
+              cnf_concurrency2 [x] [y] C \<union>\<^sub>p (cnf_concurrency2 [x] ys C \<union>\<^sub>p cnf_concurrency2 xs (y # ys) C)"
+          by (meson \<open>cnf_concurrency2 [x] ys C \<equiv>\<^sub>p evaluate (concat (map ((\<interleave>) x) ys)) C\<close> \<open>cnf_concurrency2 xs (y # ys) C \<equiv>\<^sub>p evaluate (xs \<parallel> (y # ys)) C\<close> \<open>evaluate (x \<interleave> y) C \<equiv>\<^sub>p cnf_concurrency2 [x] [y] C\<close> choice_equiv equiv_is_symetric equiv_is_transitive)
+
+        have "evaluate ((x # xs) \<parallel> (y # ys)) C = evaluate (x \<interleave> y) C \<union>\<^sub>p (evaluate (concat (map ((\<interleave>) x) ys)) C \<union>\<^sub>p evaluate (xs \<parallel> (y#ys)) C)"
+          by (simp add: \<open>(x # xs) \<parallel> (y # ys) = x \<interleave> y @ concat (map ((\<interleave>) x) ys) @ xs \<parallel> (y # ys)\<close> \<open>evaluate (x \<interleave> y @ concat (map ((\<interleave>) x) ys) @ xs \<parallel> (y # ys)) C = evaluate (x \<interleave> y) C \<union>\<^sub>p (evaluate (concat (map ((\<interleave>) x) ys)) C \<union>\<^sub>p evaluate (xs \<parallel> (y # ys)) C)\<close>)
+        have "cnf_concurrency2 (x # xs) (y # ys) C = cnf_concurrency2 [x] [y] C \<union>\<^sub>p (cnf_concurrency2 [x] ys C \<union>\<^sub>p cnf_concurrency2 xs (y # ys) C)"
+          by (metis \<open>cnf_concurrency2 (x # xs) (y # ys) C = cnf_concurrency2 (x # xx # xs') (y # yy # ys') C\<close> \<open>cnf_concurrency2 (x # xx # xs') (y # yy # ys') C = cnf_concurrency2 [x] (y # yy # ys') C \<union>\<^sub>p cnf_concurrency2 (xx # xs') (y # yy # ys') C\<close> \<open>cnf_concurrency2 [x] (y # ys) C \<union>\<^sub>p cnf_concurrency2 xs (y # ys) C = (cnf_concurrency2 [x] [y] C \<union>\<^sub>p cnf_concurrency2 [x] ys C) \<union>\<^sub>p cnf_concurrency2 xs (y # ys) C\<close> \<open>cnf_concurrency2 [x] (y # yy # ys') C \<union>\<^sub>p cnf_concurrency2 (xx # xs') (y # yy # ys') C = cnf_concurrency2 [x] (y # ys) C \<union>\<^sub>p cnf_concurrency2 xs (y # ys) C\<close> choice_assoc_1)
+        then show ?thesis
+          using \<open>evaluate ((x # xs) \<parallel> (y # ys)) C = evaluate (x \<interleave> y) C \<union>\<^sub>p (evaluate (concat (map ((\<interleave>) x) ys)) C \<union>\<^sub>p evaluate (xs \<parallel> (y # ys)) C)\<close> \<open>evaluate (x \<interleave> y) C \<union>\<^sub>p (evaluate (concat (map ((\<interleave>) x) ys)) C \<union>\<^sub>p evaluate (xs \<parallel> (y # ys)) C) \<equiv>\<^sub>p cnf_concurrency2 [x] [y] C \<union>\<^sub>p (cnf_concurrency2 [x] ys C \<union>\<^sub>p cnf_concurrency2 xs (y # ys) C)\<close> equiv_is_symetric by auto
+      qed
+    qed
+  qed
+qed
 
 end
